update

AxiomaticModel.thy
@@ -1,278 +1,316 @@
+(*Liyi Li Oct 1st, 2019 *)
+
 theory AxiomaticModel
 imports Main
 begin
 
-(* locks in the SC11 model is strange, since it locks a memory location which is impossible to implement.
-   the division between a atomic location and a non-atomic location in an execution is strange \
-  hypothetical_release_sequence definition is strange, and why rmw release can break the same thread requirement? 
-  synchorniaze-with relation too complicated and unnecessary 
-   likely that if a read of release do not read a value from a write acquire, then the SC11 model rejects
-   however, consider the following program:
-   a: write x b: fence release, thread 2: c: read x d: fence acquire, can c read value a,
-    the C11 model does not forbid c reading value from a,
-    happens-before definition is too restritive. 
-    if we require happens-before writes to satisfy modification order, then the follow program is not valid:
-     T1                T2
-    x = 1             y=1
-    a = y//a = 0      b=x//b=0
-    even if relaxed flag is given in this case, this program is disallowed according to the C11 model defined by Batty,
-    which is wrong
-
-    In a sense, the SC11 model also says very little about relaxed atomics and any relations that are not
-      in the synchronized-with relations.
-     For example, if we have
-     T1                          T2
-    x-relaxed = 1                z-relaxed = 2
-                                 y-release = 1
-    a = y-acquired //a = 0       b=x-relaxed   //b=0
-    c = z-relaxed //c = 0
-
-    it is also a valid program, but the SC11 model does not talk about thing about the behavior of the
-    program if a gets value 1, because it is not in the sw-relation.
-
-     T1                          T2                        T3
-    x-relaxed = 1                z-release = 2
-                                 y-release = 1
-    a = y-acquired //a = 0       b=x-relaxed   //b=1
-    c = z-acquired //c = 2
-
-  why need to focus on atomic/non-atomic memory locations. 
-   Does non-atomic memory operations do not need to follow modification order?
-
-   does sc read must read value from sc write? 
+(* This document is the definition file of ATRCM. 
+   An execution in ATRCM is (T,Tid,Loc,Lock,\<rho>,sbs,dds,rf):
+   A set of Time points, a finite set of thread-IDs,
+   a set of locations, a set of Lock keys,
+   a map from time points to memory events,
+   a family of sequenced-before relations (one for each thread),
+   a set of data dapendencies, and a read-from relation.
+   This model assumes that an RMW is always a single atomic element.
   *)
 
 
-
-
-
+(* syntax definition for memory order on memory operations *)
 datatype order = Relaxed | Release | Acquire | AcqRel | SeqCst
 
+(*memory actions including memory operations and fence-like structures
+  We define actions for atomic/non-atomic memory operations differently.
+  An atomic memory operation contains four field, a Boolean value for marking if the action
+  is a volatile memory operation (volatile model in LLVM), a value, a location and an order.
+  A non-atomic memory operation contains a Boolean flag for volatile memory operation flag,
+  a value, a location, an action-ID (the action-ID of the first event in the group)
+  uniquely identify a group of non-atomic memory operations
+  to be in the same group (meaning that they are from the same instruction and finishing the same task),
+  a natural number representing the i-th position of the current memory operation in the group,
+  and a natural number representing the total number of elements in the group.
+  Fence-like structures include a memory fence with order, locks, a control fence representing
+  the control dependency, and a call fence. A call fence usually comes in a pair of call fences with
+  the calling function name, and a unique key identifying the two call fences in a pair. 
+   *)
 datatype ('aid,  'val, 'loc, 'lock,'name,'key) action =
-   ARead bool 'val 'loc order "'aid list" | AWrite bool 'val 'loc order "'aid list" | RMW bool 'val 'loc order "'aid list"
-  | NRead bool 'val 'loc 'aid nat nat "'aid list" | NWrite bool 'val 'loc 'aid nat nat "'aid list"
-  | Fence order | Lock 'lock | UnLock 'lock
+    ARead bool 'val 'loc order
+  | AWrite bool 'val 'loc order
+  | RMW bool 'val 'loc order
+  | NRead bool 'val 'loc 'aid nat nat
+  | NWrite bool 'val 'loc 'aid nat nat
+  | Fence order
+  | Lock 'lock
+  | UnLock 'lock
   | CallFence 'name 'key
   | ControlFence
-  | Create 'loc
-  | Free 'loc
+
+
+(*check if a memory event's action is a write op (AWrite, RMW, NWrite) *)
+fun isWriteBasic where
+ "isWriteBasic (AWrite vol x y z) = True"
+| "isWriteBasic (RMW vol x y z) = True"
+| "isWriteBasic (NWrite vol x y z u v) = True"
+| "isWriteBasic x = False"
+
+(* check if a write is atomic *)
+fun isAtomicWriteBase where
+ "isAtomicWriteBase (AWrite vol x y z) = True"
+| "isAtomicWriteBase (RMW vol x y z) = True"
+| "isAtomicWriteBase x = False"
 
 fun isWrite where
- "isWrite (AWrite vol x y z al) = True"
-| "isWrite (RMW vol x y z al) = True"
-| "isWrite (NWrite vol x y z u v al) = True"
-| "isWrite x = False"
+ "isWrite rho t = (case rho t of None \<Rightarrow> False | Some (x,y,z) \<Rightarrow> isWriteBasic z)"
 
-fun isAtomicWrite where
- "isAtomicWrite (AWrite vol x y z al) = True"
-| "isAtomicWrite (RMW vol x y z al) = True"
-| "isAtomicWrite x = False"
+(* check if an action is a write but not a rmw *)
+fun isPureWriteBasic where
+ "isPureWriteBasic (AWrite vol x y z) = True"
+| "isPureWriteBasic (NWrite vol x y z u v) = True"
+| "isPureWriteBasic x = False"
 
-fun isWriteInTuple where
- "isWriteInTuple None = False"
-| "isWriteInTuple (Some (x,y,z)) = isWrite z"
+fun isPureWrite where
+ "isPureWrite rho t = (case rho t of None \<Rightarrow> False | Some (x,y,z) \<Rightarrow> isPureWriteBasic z)"
+
+(* check if an action is a read op ARead RMW NRead *)
+fun isReadBasic where
+"isReadBasic (ARead vol a x y) = True"
+| "isReadBasic (RMW vol x y z) = True"
+| "isReadBasic (NRead vol a x y u v) = True"
+| "isReadBasic x = False"
 
 fun isRead where
-"isRead (ARead vol a x y al) = True"
-| "isRead (RMW vol x y z al) = True"
-| "isRead (NRead vol a x y u v al) = True"
-| "isRead x = False"
+"isRead rho t = (case rho t of None \<Rightarrow> False | Some (x,y,z) \<Rightarrow> isReadBasic z)"
 
-fun isReadInTuple where
-"isReadInTuple (Some (x,y,z)) = isRead z"
-| "isReadInTuple None = False"
+(* check if an action is a read but not a rmw *)
+fun isPureReadBasic where
+"isPureReadBasic (ARead vol a x y) = True"
+| "isPureReadBasic (NRead vol a x y u v) = True"
+| "isPureReadBasic x = False"
 
 fun isPureRead where
-"isPureRead (ARead vol a x y al) = True"
-| "isPureRead (NRead vol a x y u v al) = True"
-| "isPureRead x = False"
+"isPureRead rho t = (case rho t of None \<Rightarrow> False | Some (x,y,z) \<Rightarrow> isPureReadBasic z)"
 
-fun isPureReadInTuple where
-"isPureReadInTuple (Some (x,y,z)) = isPureRead z"
-| "isPureReadInTuple None = False"
-
+(* check if an action is a memory location create 
 fun isCreate where
-"isCreate (Some (x,y,Create l)) = True"
-| "isCreate x = False"
+"isCreate rho t = (case rho t of (Some (x,y,Create l)) \<Rightarrow> True | _ \<Rightarrow> False)"
 
+ check if an action is a memory location free  
 fun isFree where
-"isFree (Some (x,y,Free l)) = True"
-| "isFree x = False"
+"isFree rho t = (case rho t of (Some (x,y,Free l)) \<Rightarrow> True | _ \<Rightarrow> False)"
+*)
 
+(* check if an action is a RMW *)
 fun isRMW where
-"isRMW (RMW vol x y z al) = True"
-| "isRMW x = False"
+"isRMW rho t = (case rho t of (Some (u,v,(RMW vol x y z))) \<Rightarrow> True | _ \<Rightarrow> False)"
 
-fun isRMWInTuple where
-"isRMWInTuple None = False"
-| "isRMWInTuple (Some (x,y,z)) = isRMW z"
-
+(* check if an action is a write or a read, a memory operation is a write or a read *)
 fun isMemOp where
- "isMemOp x = (isWrite x \<or> isPureRead x)"
+ "isMemOp rho x = (isWrite rho x \<or> isPureRead rho x)"
 
-fun isMemOpInTuple where
-"isMemOpInTuple None = False"
-| "isMemOpInTuple (Some (x,y,z)) = isMemOp z"
+(* check if an action is an atomic memory operation *)
+fun isAtomicBasic where
+ "isAtomicBasic (AWrite vol x y r) = True"
+| "isAtomicBasic (RMW vol x y r) = True"
+| "isAtomicBasic (ARead vol a x r) = True"
+| "isAtomicBasic x = False"
 
 fun isAtomic where
- "isAtomic (AWrite vol x y r al) = True"
-| "isAtomic (RMW vol x y r al) = True"
-| "isAtomic (ARead vol a x r al) = True"
-| "isAtomic x = False"
+"isAtomic rho t = (case rho t of None \<Rightarrow> False | Some (x,y,z) \<Rightarrow> isAtomicBasic z)"
 
-definition isAtomicInTuple where
-"isAtomicInTuple rho a = (case rho a of None \<Rightarrow> False | Some (x,y,z) \<Rightarrow> isAtomic z)"
+(* check if an action is a memory operation whose volatile flag is on (bool value to be true) *)
+fun isVolatileBasic where
+"isVolatileBasic (ARead vol a x y) = vol"
+| "isVolatileBasic (RMW vol x y z) = vol"
+| "isVolatileBasic (AWrite vol x y z) = vol"
+| "isVolatileBasic (NRead vol a x y u v) = vol"
+| "isVolatileBasic (NWrite vol x y z u v) = vol"
+| "isVolatileBasic x = False"
 
 fun isVolatile where
-"isVolatile (ARead vol a x y al) = vol"
-| "isVolatile (RMW vol x y z al) = vol"
-| "isVolatile (AWrite vol x y z al) = vol"
-| "isVolatile (NRead vol a x y u v al) = vol"
-| "isVolatile (NWrite vol x y z u v al) = vol"
-| "isVolatile x = False"
+"isVolatile rho t = (case rho t of None \<Rightarrow> False | Some (x,y,z) \<Rightarrow> isVolatileBasic z)"
+
+(* check if an action is an atomic memory operation whose order is SeqCst *)
+fun isSeqAtomicBasic where
+ "isSeqAtomicBasic (AWrite vol x y SeqCst) = True"
+| "isSeqAtomicBasic (RMW vol x y SeqCst) = True"
+| "isSeqAtomicBasic (ARead vol a x SeqCst) = True"
+| "isSeqAtomicBasic x = False"
 
 fun isSeqAtomic where
- "isSeqAtomic (AWrite vol x y SeqCst al) = True"
-| "isSeqAtomic (RMW vol x y SeqCst al) = True"
-| "isSeqAtomic (ARead vol a x SeqCst al) = True"
-| "isSeqAtomic x = False"
+"isSeqAtomic rho t = (case rho t of None \<Rightarrow> False | Some (x,y,z) \<Rightarrow> isSeqAtomicBasic z)"
 
-fun isSeqAtomicInTuple where
-"isSeqAtomicInTuple (Some (x,y,z)) = isSeqAtomic z"
-| "isSeqAtomicInTuple None = False"
+(* check if an action is an atomic read (ARead/rmw) whose order is SeqCst *)
+fun isSeqRead where
+"isSeqRead rho t = (isSeqAtomic rho t \<and> isRead rho t)"
 
+(* check if an action is an atomic read but not rmw  whose order is SeqCst *)
+definition isSeqPureRead where
+"isSeqPureRead rho a = (isPureRead rho a \<and> isSeqAtomic rho a)"
+
+(* check if an action is a fence whose order is SeqCst *)
 fun isSeqFence where
-"isSeqFence (Some (x,y,Fence SeqCst)) = True"
-| "isSeqFence x = False"
+"isSeqFence rho t = (case rho t of (Some (x,y,Fence SeqCst)) \<Rightarrow> True | _ \<Rightarrow> False)"
 
-fun hasSeqInTuple where
- "hasSeqInTuple x = (isSeqAtomicInTuple x \<or> isSeqFence x)"
+(* check if an action is a seqcst fence or seqcst atomic memory operation *)
+fun hasSeq where
+ "hasSeq rho x = (isSeqAtomic rho x \<or> isSeqFence rho x)"
 
+(* check if an action is a memory fence *)
 fun isRealFence where
-"isRealFence (Fence r) = True"
-| "isRealFence x = False"
+"isRealFence rho t = (case rho t of Some (x,y,(Fence r)) \<Rightarrow> True | _ \<Rightarrow> False)"
 
-definition isRealFenceInTuple where
-"isRealFenceInTuple rho x = (case rho x of None \<Rightarrow> False | (Some (u,v,w)) \<Rightarrow> isRealFence w)"
+(* check if an action is not a memory operation,
+     a fence-like structure is an action that is not a memory operation *)
+fun isFenceLikeBasic where
+"isFenceLikeBasic (Fence x) = True"
+| "isFenceLikeBasic (Lock l) = True"
+| "isFenceLikeBasic (UnLock l) = True"
+| "isFenceLikeBasic (CallFence a b) = True"
+| "isFenceLikeBasic (ControlFence) = True"
+| "isFenceLikeBasic x = False"
 
 fun isFenceLike where
-"isFenceLike (Fence x) = True"
-| "isFenceLike (Lock l) = True"
-| "isFenceLike (UnLock l) = True"
-| "isFenceLike (CallFence a b) = True"
-| "isFenceLike (ControlFence) = True"
-| "isFenceLike (Create l) = True"
-| "isFenceLike (Free l) = True"
-| "isFenceLike x = False"
-
-fun isFenceLikeTuple where
-"isFenceLikeTuple None = False"
-| "isFenceLikeTuple (Some (x,y,z)) = isFenceLike z"
+"isFenceLike rho t = (case rho t of None \<Rightarrow> False | Some (x,y,z) \<Rightarrow> isFenceLikeBasic z)"
 
 (* get the memory location of a read-write operation, and check if two ops have the same locations *)
 fun acLoc where
-"acLoc (ARead vol a x y al) = Some x"
-| "acLoc (RMW vol x y z al) = Some y"
-| "acLoc (AWrite vol x y z al) = Some y"
-| "acLoc (NRead vol a x y u v al) = Some x"
-| "acLoc (NWrite vol x y z u v al) = Some y"
-| "acLoc (Create l) = Some l"
+"acLoc (ARead vol a x y) = Some x"
+| "acLoc (RMW vol x y z) = Some y"
+| "acLoc (AWrite vol x y z) = Some y"
+| "acLoc (NRead vol a x y u v) = Some x"
+| "acLoc (NWrite vol x y z u v) = Some y"
 | "acLoc x = None"
 
-fun getLocInTuple where
-"getLocInTuple None = None"
-| "getLocInTuple (Some (x,y,z)) = acLoc z"
+fun getLoc where
+"getLoc rho t = (case rho t of None \<Rightarrow> None | Some (x,y,z) \<Rightarrow> acLoc z)"
 
+
+(* check if two memory locations from two actions are the same *)
 fun isTheLoc where
-"isTheLoc a loc = (case acLoc a of Some x \<Rightarrow> x = loc | _ \<Rightarrow> False)"
+"isTheLoc rho t loc = (case getLoc rho t of None \<Rightarrow> False | Some x \<Rightarrow> x = loc)"
 
-fun isTheLocInTuple where
-"isTheLocInTuple None loc = False"
-| "isTheLocInTuple (Some (x,y,z)) loc = isTheLoc z loc"
-
-fun sameLoc where
-"sameLoc a b  = (case acLoc a of Some x \<Rightarrow>
+fun sameLocBasic where
+"sameLocBasic a b  = (case acLoc a of Some x \<Rightarrow>
                        (case acLoc b of Some y \<Rightarrow> if x = y then True else False | _ \<Rightarrow> False)
                      | _ \<Rightarrow> False)"
 
-fun sameLocInTuple where
-"sameLocInTuple rho a b = (case rho a of None \<Rightarrow> False
+fun sameLoc where
+"sameLoc rho a b = (case rho a of None \<Rightarrow> False
                             | Some (x,y,z) \<Rightarrow> (case rho b of None \<Rightarrow> False
-                                  | Some (u,v,w) \<Rightarrow> sameLoc z w))"
+                                  | Some (u,v,w) \<Rightarrow> sameLocBasic z w))"
 
+(* get the tid of a memory event *)
+fun getTid where
+"getTid rho a = (case rho a of None \<Rightarrow> None | Some (x,y,z) \<Rightarrow> Some x)"
+
+(* check if two events being in the same thread-ID *)
 fun sameThread where
-"sameThread rho a b = (case rho a of Some (x,y,z) \<Rightarrow>
-                    (case rho b of Some (u,v,w) \<Rightarrow> if x = u then True else False
-                                 | _ \<Rightarrow> False)
-                       | _ \<Rightarrow> False)"
+"sameThread rho a b =  (case getTid rho a of None \<Rightarrow> False
+                  | Some x \<Rightarrow> (case getTid rho b of None \<Rightarrow> False | Some y \<Rightarrow> x = y))"
+
+(* get the aid (action-ID) of a memory event *)
+fun getAid where
+"getAid rho t = (case rho t of None \<Rightarrow> None | Some (x,y,z) \<Rightarrow> Some y)"
+
+(* check if two events being in the same action-ID *)
+fun sameAid where
+"sameAid rho a b = (case getAid rho a of None \<Rightarrow> False
+       | Some y \<Rightarrow> (case getAid rho b of None \<Rightarrow> False | Some z \<Rightarrow> y = z))"
 
 (* get the value of a read-write operation and check if two ops have the same value*)
 fun acVal where
-"acVal (ARead vol a x y al) = Some a"
-| "acVal (RMW vol x y z al) = Some x"
-| "acVal (AWrite vol x y z al) = Some x"
-| "acVal (NRead vol a x y u v al) = Some a"
-| "acVal (NWrite vol x y z u v al) = Some x"
+"acVal (ARead vol a x y) = Some a"
+| "acVal (RMW vol x y z) = Some x"
+| "acVal (AWrite vol x y z) = Some x"
+| "acVal (NRead vol a x y u v) = Some a"
+| "acVal (NWrite vol x y z u v) = Some x"
 | "acVal x = None"
 
-fun geValInTuple where
-"geValInTuple None = None"
-| "geValInTuple (Some (x,y,z)) = acVal z"
+fun getVal where
+"getVal rho t = (case rho t of None \<Rightarrow> None | Some (x,y,z) \<Rightarrow> acVal z)"
 
-fun sameVal where
-"sameVal a b  = (case acVal a of Some x \<Rightarrow>
+(* check if two events's actions having the same values *)
+fun sameValBasic where
+"sameValBasic a b  = (case acVal a of Some x \<Rightarrow>
                        (case acVal b of Some y \<Rightarrow> if x = y then True else False | _ \<Rightarrow> False)
                      | _ \<Rightarrow> False)"
 
-fun sameValInTuple where
-"sameValInTuple rho a b = (case rho a of None \<Rightarrow> False
+fun sameVal where
+"sameVal rho a b = (case rho a of None \<Rightarrow> False
                             | Some (x,y,z) \<Rightarrow> (case rho b of None \<Rightarrow> False
-                                  | Some (u,v,w) \<Rightarrow> sameVal z w))"
+                                  | Some (u,v,w) \<Rightarrow> sameValBasic z w))"
+
+(* get the order of an event's action *)
+fun acOrderBasic where
+"acOrderBasic (ARead vol x y z) = Some z"
+| "acOrderBasic (AWrite vol x y z) = Some z"
+| "acOrderBasic (RMW vol x y z) = Some z"
+| "acOrderBasic (Fence x) = Some x"
+| "acOrderBasic x = None"
 
 fun acOrder where
-"acOrder (ARead vol x y z al) = Some z"
-| "acOrder (AWrite vol x y z al) = Some z"
-| "acOrder (RMW vol x y z al) = Some z"
-| "acOrder (Fence x) = Some x"
-| "acOrder x = None"
+"acOrder rho t = (case rho t of None \<Rightarrow> None | Some (x,y,z) \<Rightarrow> acOrderBasic z)"
 
+(* the order of an event's action is not a relaxed *)
 definition hasAtLeastAcqRel where
-"hasAtLeastAcqRel ac = (case acOrder ac of None \<Rightarrow> False
-                                         | Some z \<Rightarrow> if z = Relaxed then False else True)"
+"hasAtLeastAcqRel rho t = (case acOrder rho t of None \<Rightarrow> False
+                               | Some z \<Rightarrow> if z = Relaxed then False else True)"
 
+(* the order of an event's action is not a relaxed or release *)
 definition atLeastAcq where
-"atLeastAcq ac = (case acOrder ac of None \<Rightarrow> False | Some z \<Rightarrow> if z = Relaxed \<or> z = Release then False else True)"
+"atLeastAcq rho t = (case acOrder rho t of None \<Rightarrow> False
+                               | Some z \<Rightarrow> if z = Relaxed \<or> z = Release then False else True)"
 
+(* the order of an event's action is not a relaxed or acquire *)
 definition atLeastRel where
-"atLeastRel ac = (case acOrder ac of None \<Rightarrow> False | Some z \<Rightarrow> if z = Relaxed \<or> z = Acquire then False else True)"
+"atLeastRel rho t = (case acOrder rho t of None \<Rightarrow> False
+                               | Some z \<Rightarrow> if z = Relaxed \<or> z = Acquire then False else True)"
 
+(* the order of an event's action is acqrel or seqcst *)
+definition atLeastAcqRel where
+"atLeastAcqRel rho t = (case acOrder rho t of None \<Rightarrow> False
+                               | Some z \<Rightarrow> if z = AcqRel \<or> z = SeqCst then True else False)"
+
+(* the order of an event's action is acquire *)
+definition isAcq where
+"isAcq rho t = (case acOrder rho t of None \<Rightarrow> False
+                               | Some z \<Rightarrow> if z = Acquire then True else False)"
+
+(* the order of an event's action is release *)
+definition isRel where
+"isRel rho t = (case acOrder rho t of None \<Rightarrow> False
+                               | Some z \<Rightarrow> if z = Release then True else False)"
+
+(* an event's action is a release write *)
 definition isRelWrite where
-"isRelWrite rho x = (case rho x of None \<Rightarrow> False | Some (u,v,w)
-                         \<Rightarrow> (isWrite w \<or> isRealFence w) \<and> atLeastRel w)"
+"isRelWrite rho x = (isRel rho x \<and> isWrite rho x)"
 
+(* an event's action is a acquire read *)
 definition isAcqRead where
-"isAcqRead rho x = (case rho x of None \<Rightarrow> False | Some (u,v,w)
-                         \<Rightarrow> (isRead w \<or> isRealFence w) \<and> atLeastAcq w)"
+"isAcqRead rho x = (isAcq rho x \<and> isRead rho x)"
 
-
+(* check if an event's action is the same as another action *)
 fun hasAction where
-"hasAction (Some (u,v,w)) y = (if w = y then True else False)"
-| "hasAction None y = False"
-
+"hasAction rho t y = (case rho t of None \<Rightarrow> False | Some (u,v,w) \<Rightarrow> (if w = y then True else False))"
 
 definition toLocalExecution where
 "toLocalExecution tid f = (\<lambda> x . (case f x of None \<Rightarrow> None | Some (a,b) \<Rightarrow> if a = tid then Some b else None))"
 
+(* get all thread ids in the co-domain of a rho *)
 definition getAllTids where
 "getAllTids f = {a . \<exists> b . (a,b) \<in> range f}"
 
+(* get the additional dependencies of an event's action (memory operation) 
+fun getDepSetBasic where
+"getDepSetBasic (ARead vol a x y al) = Some al"
+| "getDepSetBasic (RMW vol x y z al) = Some al"
+| "getDepSetBasic (AWrite vol x y z al) = Some al"
+| "getDepSetBasic (NRead vol a x y u v al) = Some al"
+| "getDepSetBasic (NWrite vol x y z u v al) = Some al"
+| "getDepSetBasic x = None"
+
 fun getDepSet where
-"getDepSet (ARead vol a x y al) = Some al"
-| "getDepSet (RMW vol x y z al) = Some al"
-| "getDepSet (AWrite vol x y z al) = Some al"
-| "getDepSet (NRead vol a x y u v al) = Some al"
-| "getDepSet (NWrite vol x y z u v al) = Some al"
-| "getDepSet x = None"
+"getDepSet rho t = (case rho t of None \<Rightarrow> None | Some (x,y,z) \<Rightarrow> getDepSetBasic z)"
+*)
 
 type_synonym loc_type = int
 type_synonym time_type = nat
@@ -296,86 +334,137 @@ locale axiomaticModel =
     and callIDs :: "'callID set"
 begin
 
-definition wellformedTime :: "time_type set \<Rightarrow>
-                    (time_type \<times> time_type) set \<Rightarrow> (time_type \<Rightarrow> ('tid \<times> aid_type \<times>
-                   (aid_type, 'val, loc_type, 'lock, 'name, 'callID) action) option) \<Rightarrow> bool" where
-"wellformedTime T rf rho = (T \<subseteq> times \<and> (\<forall> t1 t2 . (t1,t2) \<in> rf \<longrightarrow> t1 \<in> T \<and> t2 \<in> T)
-                            \<and> (\<forall> t act . rho t = Some act \<longrightarrow> t \<in> T))"
+(* 
+Here, we define some assumptions for some elements in an execution:
+(T,Tid, Loc,Lock,\<rho>,sbs,dds,rf)
+ the predicates of well-formed on time points T, tid set,
+ sbs, dds, rf, and \<rho>
+*)
+(* A well-formed T requires that it does not exist a backward edge in rf. *)
+definition wellformedTime :: "time_type set \<Rightarrow> (time_type \<Rightarrow> ('tid \<times> aid_type \<times>
+                   (aid_type, 'val, loc_type, 'lock, 'name, 'callID) action) option) \<Rightarrow>
+                    (time_type \<times> time_type) set \<Rightarrow> bool" where
+"wellformedTime T rho rf = (0 \<notin> T \<and> T \<subseteq> times \<and> (\<forall> t1 t2 . (t1,t2) \<in> rf \<longrightarrow> t1 \<in> T \<and> t2 \<in> T)
+                            \<and> (\<forall> t act . rho t = Some act \<longrightarrow> t \<in> T)
+                            \<and> (\<forall> t . t \<in> T \<longrightarrow> (\<exists> act . rho t = Some act)))"
 
+(* Well-formed assumption for the thread-ID set, as every event in \<rho> should be a valid thread-ID. *)
 definition wellformedTid :: "'tid set \<Rightarrow> (time_type \<Rightarrow> ('tid \<times> aid_type \<times>
                    (aid_type, 'val, loc_type, 'lock, 'name, 'callID) action) option) \<Rightarrow> bool" where
 "wellformedTid Tid rho = (Tid \<subseteq> threads \<and>
                             (\<forall> t tid aid ac . rho t = Some (tid,aid,ac) \<longrightarrow> tid \<in> Tid))"
 
-definition wellformedSB :: "'tid set \<Rightarrow> time_type set \<Rightarrow> ('tid \<Rightarrow> (time_type \<times> time_type) set option) \<Rightarrow> bool" where
-"wellformedSB Tid T sb = (\<forall> t S a b . sb t = Some S \<and> (a,b) \<in> S \<longrightarrow> t \<in> Tid \<and> a \<in> T \<and> b \<in> T)"
+(* Well-formed assumption for sbs, such that every time points in the relation must be a valid one in T *)
+definition wellformedSB1 :: "'tid set \<Rightarrow> time_type set
+                                      \<Rightarrow> ('tid \<Rightarrow> (time_type \<times> time_type) set option) \<Rightarrow> bool" where
+"wellformedSB1 Tid T sbs = (\<forall> t S a b . sbs t = Some S \<and> (a,b) \<in> S \<longrightarrow> t \<in> Tid \<and> a \<in> T \<and> b \<in> T)"
+
+(* each sb in sbs also needs to be disjointedly unioned.*)
+definition wellformedSB2 :: "'tid set \<Rightarrow> time_type set
+                                      \<Rightarrow> ('tid \<Rightarrow> (time_type \<times> time_type) set option) \<Rightarrow> bool" where
+"wellformedSB2 Tid T sbs = (\<forall> t1 t2 S1 S2 . t1 \<noteq> t2 \<and> sbs t1 = Some S1 \<and> sbs t2 = Some S2
+                            \<longrightarrow> Field (S1) \<inter> Field (S2) = {})"
+definition wellformedSB where
+"wellformedSB Tid T sbs = (wellformedSB1 Tid T sbs \<and> wellformedSB2 Tid T sbs)"
+
+(* all relations of dds should be contained in sbs, so it is obviously dds \<union> sbs+ is acyclic.*)
+definition wellformedDD where
+"wellformedDD Tid sbs dds = (\<forall> tid . trancl (the (dds tid)) \<subseteq> trancl (the (sbs tid)))"
+
+(* Well-formed rf needs to satisfy that for every pair (a,b) in rf, 
+   a is a time point of write, while b is a time point of read. *)
+definition wellformedRF where
+"wellformedRF T rho rf = ((\<forall> a b . (a,b) \<in> rf \<longrightarrow> a \<in> T \<and> b \<in> T)
+                       \<and> (\<forall> a b . (a,b) \<in> rf \<longrightarrow> isWrite rho a \<and> isRead rho b \<and> sameLoc rho a b))"
+
+definition rfAssumption :: "(time_type \<times> time_type) set
+                          \<Rightarrow> (time_type \<Rightarrow> ('tid \<times> aid_type \<times>
+                   (aid_type, 'val, loc_type, 'lock, 'name, 'callID) action) option) \<Rightarrow> bool" where
+"rfAssumption rf rho = ((\<forall> a b . (a,b) \<in> rf
+        \<longrightarrow> isWrite rho a \<and> isRead rho b \<and> sameLoc rho a b \<and> a < b \<and> sameVal rho a b) \<and>
+          (\<forall> a1 a2 b .  (a1,b) \<in> rf \<and> (a2,b) \<in> rf \<longrightarrow> (a1 = a2)))"
+
 
 definition sbAssumption :: "(time_type \<times> time_type) set
                           \<Rightarrow> (time_type \<Rightarrow> ('tid \<times> aid_type \<times>
                    (aid_type, 'val, loc_type, 'lock, 'name, 'callID) action) option) \<Rightarrow> bool" where
-"sbAssumption sb rho = (\<forall> a b tid aid1 ac1 aid2 ac2 . (a,b) \<in> sb \<longrightarrow>
-           rho a = Some (tid, aid1,ac1) \<and> rho b = Some (tid, aid2,ac2)
+"sbAssumption sb rho = (\<forall> a b aid1 aid2  . (a,b) \<in> sb \<longrightarrow>
+           getAid rho a = Some aid1 \<and> getAid rho b = Some aid2 \<and> sameThread rho a b
              \<and> aid1 < aid2 \<and> \<not> (\<exists> z . aid1 < z \<and> z < aid2))"
 
+(* The following two assumptions assume that the order of a group of non-atomic events
+   is in the increasing of the order of the position number of the non-atomic actions of the events.
+   This assumption is just for simplicity.  *)
 definition sbNReadAssumption :: "(time_type \<times> time_type) set
                           \<Rightarrow> (time_type \<Rightarrow> ('tid \<times> aid_type \<times>
                    (aid_type, 'val, loc_type, 'lock, 'name, 'callID) action) option) \<Rightarrow> bool" where
-"sbNReadAssumption sb rho = (\<forall> a b tid1 aid1  tid2 aid2 x t na nb n v v' al vol . (a,b) \<in> trancl sb \<and>
-           rho a = Some (tid1, aid1, NRead vol v x t na n al) \<and> rho b = Some (tid2,aid2,NRead vol v' x t nb n al)
+"sbNReadAssumption sb rho = (\<forall> a b tid1 aid1  tid2 aid2 x t na nb n v v' vol . (a,b) \<in> trancl sb \<and>
+           rho a = Some (tid1, aid1, NRead vol v x t na n) \<and> rho b = Some (tid2,aid2,NRead vol v' x t nb n)
              \<and> a < b \<longrightarrow> na < nb)"
 
 definition sbNWriteAssumption :: "(time_type \<times> time_type) set
                           \<Rightarrow> (time_type \<Rightarrow> ('tid \<times> aid_type \<times>
                    (aid_type, 'val, loc_type, 'lock, 'name, 'callID) action) option) \<Rightarrow> bool" where
-"sbNWriteAssumption sb rho = (\<forall> a b tid1 aid1  tid2 aid2 v1 v2 x t na nb n al vol . (a,b) \<in> trancl sb \<and>
-           rho a = Some (tid1, aid1, NWrite vol v1 x t na n al) \<and> rho b = Some (tid2,aid2,NWrite vol v2 x t nb n al)
+"sbNWriteAssumption sb rho = (\<forall> a b tid1 aid1  tid2 aid2 v1 v2 x t na nb n vol . (a,b) \<in> trancl sb \<and>
+           rho a = Some (tid1, aid1, NWrite vol v1 x t na n) \<and> rho b = Some (tid2,aid2,NWrite vol v2 x t nb n)
              \<and> a < b \<longrightarrow> na < nb)"
 
 definition sbAllAssumptions where
 "sbAllAssumptions sb rho = (sbAssumption sb rho \<and> sbNReadAssumption sb rho \<and> sbNWriteAssumption sb rho)"
 
-definition rhoAssumption :: "(time_type \<Rightarrow> ('tid \<times> aid_type \<times>
-                   (aid_type, 'val, loc_type, 'lock, 'name, 'callID) action) option) \<Rightarrow> bool" where
-"rhoAssumption rho = (\<forall> t t1 tid aid ac tid1 ac1 . t \<in> times \<and> t1 \<in> times \<and> rho t = Some (tid, aid, ac)
-                      \<and> rho t1 = Some (tid1, aid, ac1) \<longrightarrow> t = t1)"
+definition allSbAllAssumptions where
+"allSbAllAssumptions Tids sbs rho = (\<forall> tid \<in> Tids .
+                        (\<forall> sb . sbs tid = Some sb \<longrightarrow> sbAllAssumptions sb rho))"
 
-definition rfAssumption :: "(time_type \<times> time_type) set
-                          \<Rightarrow> (time_type \<Rightarrow> ('tid \<times> aid_type \<times>
-                   (aid_type, 'val, loc_type, 'lock, 'name, 'callID) action) option) \<Rightarrow> bool" where
-"rfAssumption rf rho = ((\<forall> a b tid1 aid1 ac1 tid2 aid2 ac2 . (a,b) \<in> rf
-        \<longrightarrow> rho a = Some (tid1, aid1, ac1) \<and> rho b = Some (tid2, aid2, ac2)
-           \<and> isWrite ac1 \<and> isRead ac2 \<and> sameLoc ac1 ac2 \<and> a < b \<and> sameVal ac1 ac2) \<and>
-          (\<forall> a1 a2 b .  (a1,b) \<in> rf \<and> (a2,b) \<in> rf \<longrightarrow> (a1 = a2)))"
+(* The assumption about the range of \<rho>. The domain of it is larger than T,
+    and there is a unique action id for every event in the range of \<rho>. *)
+definition rhoAssumption where
+"rhoAssumption T rho = (rho 0 = None
+          \<and> (\<forall> t t1  . t \<in> T \<and> t1 \<in> T \<and> sameAid rho t t1 \<longrightarrow> t = t1) \<and> T \<subseteq> dom rho)"
 
+(*These two assumptions restricts the write-read pairs of non-atomic operations in rf. 
+  We assume that in an execution,
+   a write-read pair including a non-atomic memory operation happens iff
+   every event in the group of the non-atomic operations happens in the execution, 
+    and only the non-atomic memory operation in the group with its position number and ttoal
+    the same can join the communication as an element of a pair in rf.
+    Combining this assumption with the above assumptions that non-atomic
+    operations must come in order, it means that only the last memory operation of a group of
+    non-atomic operations can join the communication in a rf in an execution.
+  This can be turned into a relation in the model to select valid candidate executions,
+  so that the non-satisfied executions can be viewed as a communication having a race
+   since there is a non-atomic instruction that does not finish all messages sending. 
+   At this point, we just leave it as an assumption.  *)
 definition rfNWriteAssumption :: "(time_type \<times> time_type) set
                           \<Rightarrow> (time_type \<Rightarrow> ('tid \<times> aid_type \<times>
                    (aid_type, 'val, loc_type, 'lock, 'name, 'callID) action) option) \<Rightarrow> bool" where
-"rfNWriteAssumption rf rho = (\<forall> a b tid1 aid1 v x t na n al vol . (a,b) \<in> rf
-        \<and> rho a = Some (tid1, aid1, NWrite vol v x t na n al)  \<longrightarrow> na = n)"
+"rfNWriteAssumption rf rho = (\<forall> a b tid1 aid1 v x t na n vol . (a,b) \<in> rf
+        \<and> rho a = Some (tid1, aid1, NWrite vol v x t na n)  \<longrightarrow> na = n)"
 
 definition rfNReadAssumption :: "(time_type \<times> time_type) set
                           \<Rightarrow> (time_type \<Rightarrow> ('tid \<times> aid_type \<times>
                    (aid_type, 'val, loc_type, 'lock, 'name, 'callID) action) option) \<Rightarrow> bool" where
-"rfNReadAssumption rf rho = (\<forall> a b tid1 aid1 x t na n v al vol . (a,b) \<in> rf
-        \<and> rho b = Some (tid1, aid1, NRead vol v x t na n al)  \<longrightarrow> na = n)"
+"rfNReadAssumption rf rho = (\<forall> a b tid1 aid1 x t na n v vol . (a,b) \<in> rf
+        \<and> rho b = Some (tid1, aid1, NRead vol v x t na n)  \<longrightarrow> na = n)"
 
 definition rfAllAssumption where
 "rfAllAssumption rf rho = (rfAssumption rf rho \<and> rfNWriteAssumption rf rho \<and> rfNReadAssumption rf rho)"
 
-(* defining a relation collecting the sb-position relation on all fence like ops in each thread *)
+(* defining a relation collecting the sb-position relation on all fence-like ops in each thread
+   This relation set all fences not crossing each other in an execution. *)
 inductive_set fenceRelation :: "time_type set 
     \<Rightarrow> (time_type \<Rightarrow> ('tid \<times> aid_type \<times>
                    (aid_type, 'val, loc_type, 'lock, 'name, 'callID) action) option) \<Rightarrow>
               (time_type \<times> time_type) set
           \<Rightarrow> (time_type \<times> time_type) set"
-  for E :: "time_type set"
+  for T :: "time_type set"
     and rho :: "(time_type \<Rightarrow> ('tid \<times> aid_type \<times>
                    (aid_type, 'val, loc_type, 'lock, 'name, 'callID) action) option)"
     and sb :: "(time_type \<times> time_type) set" 
   where
   fenceLikeRule : "\<lbrakk> (a,b) \<in> trancl sb;
-               isFenceLikeTuple (rho a); isFenceLikeTuple (rho b)\<rbrakk>
-           \<Longrightarrow> (a,b) \<in> fenceRelation E rho sb"
+               isFenceLike rho a; isFenceLike rho b\<rbrakk>
+           \<Longrightarrow> (a,b) \<in> fenceRelation T rho sb"
 
 (* defining control dependence,
    control dependence happens when there is a binary branching inst in the time of the op. 
@@ -386,19 +475,19 @@ inductive_set controldep :: "time_type set
                    (aid_type, 'val, loc_type, 'lock, 'name, 'callID) action) option) \<Rightarrow>
               (time_type \<times> time_type) set
           \<Rightarrow> (time_type \<times> time_type) set"
-  for E :: "time_type set"
+  for T :: "time_type set"
     and rho :: "(time_type \<Rightarrow> ('tid \<times> aid_type \<times>
                    (aid_type, 'val, loc_type, 'lock, 'name, 'callID) action) option)"
     and sb :: "(time_type \<times> time_type) set" 
   where
   controlWriteRule1: "\<lbrakk> (a,b) \<in> trancl sb;
-             rho b = Some (tid, aid, ControlFence); {a,b} \<subseteq> E; isWriteInTuple (rho a)\<rbrakk>
-           \<Longrightarrow> (a,b) \<in> controldep E rho sb"
+             rho b = Some (tid, aid, ControlFence); {a,b} \<subseteq> T; isWrite rho a\<rbrakk>
+           \<Longrightarrow> (a,b) \<in> controldep T rho sb"
 | controlWriteRule2: "\<lbrakk> (a,b) \<in> trancl sb;
-             rho a = Some (tid, aid, ControlFence); {a,b} \<subseteq> E; isWriteInTuple (rho b)\<rbrakk>
-           \<Longrightarrow> (a,b) \<in> controldep E rho sb"
+             rho a = Some (tid, aid, ControlFence); {a,b} \<subseteq> T; isWrite rho b\<rbrakk>
+           \<Longrightarrow> (a,b) \<in> controldep T rho sb"
 
-(* call dependency is like a acqrel fence in each thread to indicate that
+(* call/lock dependency is like a acqrel fence in each thread to indicate that
     a memory op cannot go cross a function call (lib call). 
    this fence is useful in doing function call optimization
    i.e. declaring a function is an inline function *)
@@ -406,44 +495,56 @@ inductive_set calldep :: "time_type set  \<Rightarrow> (time_type \<Rightarrow> 
                    (aid_type, 'val, loc_type, 'lock, 'name, 'callID) action) option) \<Rightarrow>
               (time_type \<times> time_type) set
           \<Rightarrow> (time_type \<times> time_type) set"
-  for E :: "time_type set"
+  for T :: "time_type set"
     and rho :: "(time_type \<Rightarrow> ('tid \<times> aid_type \<times>
                    (aid_type, 'val, loc_type, 'lock, 'name, 'callID) action) option)"
     and sb :: "(time_type \<times> time_type) set" 
   where
-  callFence1: "\<lbrakk> (a,b) \<in> trancl sb; rho b = Some (tid,aid,CallFence name key); {a,b} \<subseteq> E;
-                    isMemOpInTuple (rho a)\<rbrakk>
+  callFence1: "\<lbrakk> (a,b) \<in> trancl sb; rho b = Some (tid,aid,CallFence name key);
+                    isMemOp rho a \<rbrakk>
+           \<Longrightarrow> (a,b) \<in> calldep T rho sb"
+| callFence2: "\<lbrakk> (a,b) \<in> trancl sb; rho a = Some (tid,aid,CallFence name key);
+                isMemOp rho b\<rbrakk>
+           \<Longrightarrow> (a,b) \<in> calldep T rho sb"
+| lockRule1: "\<lbrakk> (a,b) \<in> trancl sb; rho b = Some (tid, aid, (Lock l));
+                isMemOp rho a\<rbrakk>
+           \<Longrightarrow> (a,b) \<in> calldep T rho sb"
+| lockRule2: "\<lbrakk> (a,b) \<in> trancl sb; rho a = Some (tid, aid, (Lock l));
+                isMemOp rho b\<rbrakk>
+           \<Longrightarrow> (a,b) \<in> calldep T rho sb"
+| unLockRule1: "\<lbrakk> (a,b) \<in> trancl sb; rho b = Some (tid,aid,(UnLock l));
+                   isMemOp rho a\<rbrakk>
+           \<Longrightarrow> (a,b) \<in> calldep T rho sb"
+| unLockRule2: "\<lbrakk> (a,b) \<in> trancl sb; rho a = Some (tid,aid,(UnLock l));
+                   isMemOp rho b\<rbrakk>
+           \<Longrightarrow> (a,b) \<in> calldep T rho sb"
+(*| createRule1: "\<lbrakk> (a,b) \<in> trancl sb; isCreate rho b; {a,b} \<subseteq> E; isMemOp rho a\<rbrakk>
            \<Longrightarrow> (a,b) \<in> calldep E rho sb"
-| callFence2: "\<lbrakk> (a,b) \<in> trancl sb; rho a = Some (tid,aid,CallFence name key); {a,b} \<subseteq> E;
-                isMemOpInTuple (rho b)\<rbrakk>
+| createRule2: "\<lbrakk> (a,b) \<in> trancl sb; isCreate rho a;{a,b} \<subseteq> E;isMemOp rho b\<rbrakk>
            \<Longrightarrow> (a,b) \<in> calldep E rho sb"
-| lockRule1: "\<lbrakk> (a,b) \<in> trancl sb; rho b = Some (tid, aid, (Lock l)); {a,b} \<subseteq> E;
-                isMemOpInTuple (rho a)\<rbrakk>
+| freeRule1: "\<lbrakk> (a,b) \<in> trancl sb; isFree rho b; {a,b} \<subseteq> E; isMemOp rho a\<rbrakk>
            \<Longrightarrow> (a,b) \<in> calldep E rho sb"
-| lockRule2: "\<lbrakk> (a,b) \<in> trancl sb; rho a = Some (tid, aid, (Lock l)); {a,b} \<subseteq> E;
-                isMemOpInTuple (rho b)\<rbrakk>
-           \<Longrightarrow> (a,b) \<in> calldep E rho sb"
-| unLockRule1: "\<lbrakk> (a,b) \<in> trancl sb; rho b = Some (tid,aid,(UnLock l)); {a,b} \<subseteq> E;
-                   isMemOpInTuple (rho a)\<rbrakk>
-           \<Longrightarrow> (a,b) \<in> calldep E rho sb"
-| unLockRule2: "\<lbrakk> (a,b) \<in> trancl sb; rho a = Some (tid,aid,(UnLock l)); {a,b} \<subseteq> E;
-                    isMemOpInTuple (rho b)\<rbrakk>
-           \<Longrightarrow> (a,b) \<in> calldep E rho sb"
+| freeRule2: "\<lbrakk> (a,b) \<in> trancl sb; isFree rho a; {a,b} \<subseteq> E; isMemOp rho b\<rbrakk>
+           \<Longrightarrow> (a,b) \<in> calldep E rho sb" *)
 
-(* volatile dependency in all threads *)
+(* volatile dependency in all threads.
+   LLVM volatile model indicates that any two volatile memory operations cannot switch order. *)
 inductive_set volatileDep :: "time_type set  \<Rightarrow> (time_type \<Rightarrow> ('tid \<times> aid_type \<times>
                    (aid_type, 'val, loc_type, 'lock, 'name, 'callID) action) option) \<Rightarrow>
               (time_type \<times> time_type) set \<Rightarrow> (time_type \<times> time_type) set"
-  for E :: "time_type set"
+  for T :: "time_type set"
     and rho :: "(time_type \<Rightarrow> ('tid \<times> aid_type \<times>
                    (aid_type, 'val, loc_type, 'lock, 'name, 'callID) action) option)"
     and sb :: "(time_type \<times> time_type) set" 
   where
- volDef : "\<lbrakk> (a,b) \<in> trancl sb; rho a = Some (tida,aida,aca);
-                    (rho b) = Some (tidb,aidb,acb); {a,b} \<subseteq> E; isVolatile aca; isVolatile acb \<rbrakk>
-           \<Longrightarrow> (a,b) \<in> volatileDep E rho sb"
+ volDef : "\<lbrakk> (a,b) \<in> trancl sb; isVolatile rho a; isVolatile rho b \<rbrakk>
+           \<Longrightarrow> (a,b) \<in> volatileDep T rho sb"
 
-(* define data dependency in all threads *)
+(* define data dependency in all threads and additional dependencies.
+   Another way of defining data dependency by compiling additional data dependency
+   on memory operations and having basic dependency from the relations of different
+   memory operations. It will be a simpler proof for connecting ATRCM with the LLVM operational model.
+
 inductive_set addDataDep :: "time_type set  \<Rightarrow> (time_type \<Rightarrow> ('tid \<times> aid_type \<times>
                    (aid_type, 'val, loc_type, 'lock, 'name, 'callID) action) option) \<Rightarrow>
               (time_type \<times> time_type) set \<Rightarrow> (time_type \<times> time_type) set"
@@ -452,9 +553,10 @@ inductive_set addDataDep :: "time_type set  \<Rightarrow> (time_type \<Rightarro
                    (aid_type, 'val, loc_type, 'lock, 'name, 'callID) action) option)"
     and sb :: "(time_type \<times> time_type) set" 
   where
- additionalDep : "\<lbrakk> (a,b) \<in> trancl sb; rho a = Some (tida,aida,aca);
-                    (rho b) = Some (tidb,aidb,acb); {a,b} \<subseteq> E; getDepSet acb = Some al; aida \<in> set al\<rbrakk>
+ additionalDep : "\<lbrakk> (a,b) \<in> trancl sb; {a,b} \<subseteq> E; getDepSet rho b = Some bl;
+                     getAid rho a = Some aid; aid \<in> set bl\<rbrakk>
            \<Longrightarrow> (a,b) \<in> addDataDep E rho sb"
+
 
 inductive_set basicDatadep :: "time_type set  \<Rightarrow> (time_type \<Rightarrow> ('tid \<times> aid_type \<times>
                    (aid_type, 'val, loc_type, 'lock, 'name, 'callID) action) option) \<Rightarrow>
@@ -464,114 +566,92 @@ inductive_set basicDatadep :: "time_type set  \<Rightarrow> (time_type \<Rightar
                    (aid_type, 'val, loc_type, 'lock, 'name, 'callID) action) option)"
     and sb :: "(time_type \<times> time_type) set" 
   where
-  wwdependence: "\<lbrakk> (a,b) \<in> trancl sb; rho a = Some (tida,aida,aca);
-                    (rho b) = Some (tidb,aidb,acb); {a,b} \<subseteq> E; isWrite aca; isWrite acb; sameLoc aca acb\<rbrakk>
+  wwdependence: "\<lbrakk> (a,b) \<in> trancl sb;  {a,b} \<subseteq> E; isWrite rho a; isWrite rho b; sameLoc rho a b\<rbrakk>
            \<Longrightarrow> (a,b) \<in> basicDatadep E rho sb"
-| rwdependence: "\<lbrakk> (a,b) \<in> trancl sb; rho a = Some (tida,aida,aca);
-              rho b = Some (tidb,aidb,acb); {a,b} \<subseteq> E; isRead aca; \<not> isRMW aca; isWrite acb; sameLoc aca acb\<rbrakk>
+| rwdependence: "\<lbrakk> (a,b) \<in> trancl sb; {a,b} \<subseteq> E; isPureRead rho a; isWrite rho b; sameLoc rho a b\<rbrakk>
            \<Longrightarrow> (a,b) \<in> basicDatadep E rho sb"
-| wrdependence: "\<lbrakk> (a,b) \<in> trancl sb; rho a = Some (tida,aida,aca);
-              rho b = Some (tidb,aidb,acb); {a,b} \<subseteq> E; isWrite aca; isRead acb; \<not> isRMW acb; sameLoc aca acb\<rbrakk>
+| wrdependence: "\<lbrakk> (a,b) \<in> trancl sb; {a,b} \<subseteq> E; isWrite rho a; isPureRead rho b; sameLoc rho a b\<rbrakk>
            \<Longrightarrow> (a,b) \<in> basicDatadep E rho sb"
 
 definition datadep where
 "datadep E rho sb = (addDataDep E rho sb) \<union> basicDatadep E rho sb"
+*)
 
-(* memory ordering dependency in a single thread *)
+(* memory ordering dependency in a single thread.
+   Most memory orders except SeqCst order only have single-threaded effects.
+   The current seqcst + read or seqcst + write operations are too weak
+   according to the C++ documentation. Needs the version here to match RC11. *)
 inductive_set singleorderdep :: "time_type set \<Rightarrow> (time_type \<Rightarrow> ('tid \<times> aid_type \<times>
                    (aid_type, 'val, loc_type, 'lock, 'name, 'callID) action) option) \<Rightarrow>
               (time_type \<times> time_type) set
           \<Rightarrow> (time_type \<times> time_type) set"
-  for E :: "time_type set"
+  for T :: "time_type set"
     and rho :: " (time_type \<Rightarrow> ('tid \<times> aid_type \<times>
                    (aid_type, 'val, loc_type, 'lock, 'name, 'callID) action) option)"
     and sb :: "(time_type \<times> time_type) set" where
-  readAcqRule: "\<lbrakk> (a,b) \<in> trancl sb; (rho a) = Some (tid1,aid1, (ARead vol val x or axl));
-                      or = Acquire;  {a,b} \<subseteq> E;
-                  rho b = Some (tid2,aid2,ac2); isWrite ac2 \<or> isRead ac2\<rbrakk>
-           \<Longrightarrow> (a,b) \<in> singleorderdep E rho sb"
-| readSeqRule1: "\<lbrakk> (a,b) \<in> trancl sb; (rho a) = Some (tid1,aid1, (ARead vol val x or axl ));
-                      or = SeqCst;  {a,b} \<subseteq> E;
-                  rho b = Some (tid2,aid2,ac2); isWrite ac2 \<or> isRead ac2\<rbrakk>
-           \<Longrightarrow> (a,b) \<in> singleorderdep E rho sb"
-| readSeqRule2: "\<lbrakk> (a,b) \<in> trancl sb; (rho b) = Some (tid1,aid1, (ARead vol val x or axl));
-                      or = SeqCst;  {a,b} \<subseteq> E;
-                  rho a = Some (tid2,aid2,ac2); isWrite ac2\<rbrakk>
-           \<Longrightarrow> (a,b) \<in> singleorderdep E rho sb"
-| writeRelRule: "\<lbrakk> (a,b) \<in> trancl sb; (rho b) = Some (tid1,aid1,AWrite vol v x or axl);
-                       or = Release; {a,b} \<subseteq> E;
-                  rho a = Some (tid2,aid2,ac2); isWrite ac2 \<or> isRead ac2\<rbrakk>
-           \<Longrightarrow> (a,b) \<in> singleorderdep E rho sb"
-| writeSeqRule1: "\<lbrakk> (a,b) \<in> trancl sb; (rho b) = Some (tid1,aid1,AWrite vol v x or axl);
-                       or = SeqCst; {a,b} \<subseteq> E;
-                  rho a = Some (tid2,aid2,ac2); isWrite ac2 \<or> isRead ac2\<rbrakk>
-           \<Longrightarrow> (a,b) \<in> singleorderdep E rho sb"
-| writeSeqRule2: "\<lbrakk> (a,b) \<in> trancl sb; (rho a) = Some (tid1,aid1,AWrite vol v x or axl);
-                       or = SeqCst; {a,b} \<subseteq> E;
-                  rho b = Some (tid2,aid2,ac2); isWrite ac2\<rbrakk>
-           \<Longrightarrow> (a,b) \<in> singleorderdep E rho sb"
-| rmwAcqRule: "\<lbrakk> (a,b) \<in> trancl sb; (rho a) = Some (tid1,aid1, RMW vol v x or axl);
-                   or = Acquire; {a,b} \<subseteq> E;
-                  rho b = Some (tid2,aid2,ac2); isWrite ac2 \<or> isRead ac2\<rbrakk>
-           \<Longrightarrow> (a,b) \<in> singleorderdep E rho sb"
-| rmwRelRule: "\<lbrakk> (a,b) \<in> trancl sb; (rho b) = Some (tid1,aid1,RMW vol v x or axl);
-                    or = Release; {a,b} \<subseteq> E;
-                  rho a = Some (tid2,aid2,ac2); isWrite ac2 \<or> isRead ac2\<rbrakk>
-           \<Longrightarrow> (a,b) \<in> singleorderdep E rho sb"
-| rmwAllRule1: "\<lbrakk> (a,b) \<in> trancl sb; (rho b) = Some (tid1,aid1,RMW vol v x or axl);
-                       or = AcqRel \<or> or = SeqCst; {a,b} \<subseteq> E;
-                  rho a = Some (tid2,aid2,ac2); isWrite ac2 \<or> isRead ac2\<rbrakk>
-           \<Longrightarrow> (a,b) \<in> singleorderdep E rho sb"
-| rmwAllRule2: "\<lbrakk> (a,b) \<in> trancl sb; (rho a) = Some (tid1,aid1,RMW vol v x or axl);
-                     or = AcqRel \<or> or = SeqCst; {a,b} \<subseteq> E;
-                  rho b = Some (tid2,aid2,ac2); isWrite ac2 \<or> isRead ac2\<rbrakk>
-           \<Longrightarrow> (a,b) \<in> singleorderdep E rho sb"
-| acqFence1 : "\<lbrakk> (a,b) \<in> trancl sb; (rho a) = Some (tid1,aid1,Fence Acquire); {a,b} \<subseteq> E;
-                  rho b = Some (tid2,aid2,ac2); isWrite ac2 \<or> isRead ac2\<rbrakk>
-           \<Longrightarrow> (a,b) \<in> singleorderdep E rho sb"
-| acqFence2 : "\<lbrakk> (a,b) \<in> trancl sb; (rho b) = Some (tid1,aid1,Fence Acquire); {a,b} \<subseteq> E;
-                  rho a = Some (tid2,aid2,ac2); isRead ac2\<rbrakk>
-           \<Longrightarrow> (a,b) \<in> singleorderdep E rho sb"
-| relFence1 : "\<lbrakk> (a,b) \<in> trancl sb; (rho b) = Some (tid1,aid1,Fence Release); {a,b} \<subseteq> E;
-                  rho a = Some (tid2,aid2,ac2); isWrite ac2 \<or> isRead ac2\<rbrakk>
-           \<Longrightarrow> (a,b) \<in> singleorderdep E rho sb"
-| relFence2 : "\<lbrakk> (a,b) \<in> trancl sb; (rho a) = Some (tid1,aid1,Fence Release); {a,b} \<subseteq> E;
-                  rho b = Some (tid2,aid2,ac2); isWrite ac2\<rbrakk>
-           \<Longrightarrow> (a,b) \<in> singleorderdep E rho sb"
-| acqRelFence1 : "\<lbrakk> (a,b) \<in> trancl sb; (rho b) = Some (tid1,aid1,Fence AcqRel); {a,b} \<subseteq> E;
-                  rho a = Some (tid2,aid2,ac2); isWrite ac2 \<or> isRead ac2\<rbrakk>
-           \<Longrightarrow> (a,b) \<in> singleorderdep E rho sb"
-| acqRelFence2 : "\<lbrakk> (a,b) \<in> trancl sb; (rho a) = Some (tid1,aid1,Fence AcqRel); {a,b} \<subseteq> E;
-                  rho b = Some (tid2,aid2,ac2); isWrite ac2 \<or> isRead ac2\<rbrakk>
-           \<Longrightarrow> (a,b) \<in> singleorderdep E rho sb"
-| seqFence1 : "\<lbrakk> (a,b) \<in> trancl sb; (rho b) = Some (tid1,aid1,Fence SeqCst); {a,b} \<subseteq> E;
-                  rho a = Some (tid2,aid2,ac2); isWrite ac2 \<or> isRead ac2\<rbrakk>
-           \<Longrightarrow> (a,b) \<in> singleorderdep E rho sb"
-| seqFence2 : "\<lbrakk> (a,b) \<in> trancl sb; (rho a) = Some (tid1,aid1,Fence SeqCst); {a,b} \<subseteq> E;
-                  rho b = Some (tid2,aid2,ac2); isWrite ac2 \<or> isRead ac2\<rbrakk>
-           \<Longrightarrow> (a,b) \<in> singleorderdep E rho sb"
+  readAcqRule: "\<lbrakk> (a,b) \<in> trancl sb; isAcqRead rho a;
+                  isWrite rho b \<or> isPureRead rho b\<rbrakk>
+           \<Longrightarrow> (a,b) \<in> singleorderdep T rho sb"
+| readSeqRule1: "\<lbrakk> (a,b) \<in> trancl sb; isSeqAtomic rho a; isPureRead rho a; 
+                   isWrite rho b \<or> isRead rho b\<rbrakk>
+           \<Longrightarrow> (a,b) \<in> singleorderdep T rho sb"
+| readSeqRule2: "\<lbrakk> (a,b) \<in> trancl sb; isSeqAtomic rho b; isPureRead rho b; isWrite rho a\<rbrakk>
+           \<Longrightarrow> (a,b) \<in> singleorderdep T rho sb"
+| writeRelRule: "\<lbrakk> (a,b) \<in> trancl sb; isRelWrite rho b;{a,b} \<subseteq> E;
+                  isWrite rho a \<or> isRead rho a\<rbrakk>
+           \<Longrightarrow> (a,b) \<in> singleorderdep T rho sb"
+| writeSeqRule1: "\<lbrakk> (a,b) \<in> trancl sb; isPureWrite rho b; isSeqAtomic rho b; {a,b} \<subseteq> E;
+                     isWrite rho a \<or> isRead rho a\<rbrakk>
+           \<Longrightarrow> (a,b) \<in> singleorderdep T rho sb"
+| writeSeqRule2: "\<lbrakk> (a,b) \<in> trancl sb; isPureWrite rho a; isSeqAtomic rho a;
+                     isWrite rho b \<rbrakk>
+           \<Longrightarrow> (a,b) \<in> singleorderdep T rho sb"
+| rmwAllRule1: "\<lbrakk> (a,b) \<in> trancl sb; isRMW rho b; atLeastAcqRel rho b; isMemOp rho a\<rbrakk>
+           \<Longrightarrow> (a,b) \<in> singleorderdep T rho sb"
+| rmwAllRule2: "\<lbrakk> (a,b) \<in> trancl sb; isRMW rho a; atLeastAcqRel rho a; isMemOp rho b\<rbrakk>
+           \<Longrightarrow> (a,b) \<in> singleorderdep T rho sb"
+| acqFence1 : "\<lbrakk> (a,b) \<in> trancl sb; isRealFence rho a; isAcq rho a; isMemOp rho b\<rbrakk>
+           \<Longrightarrow> (a,b) \<in> singleorderdep T rho sb"
+| acqFence2 : "\<lbrakk> (a,b) \<in> trancl sb; isRealFence rho b; isAcq rho b;isRead rho a\<rbrakk>
+           \<Longrightarrow> (a,b) \<in> singleorderdep T rho sb"
+| relFence1 : "\<lbrakk> (a,b) \<in> trancl sb; isRealFence rho b; isRel rho b; isMemOp rho a\<rbrakk>
+           \<Longrightarrow> (a,b) \<in> singleorderdep T rho sb"
+| relFence2 : "\<lbrakk> (a,b) \<in> trancl sb; isRealFence rho a; isRel rho a; isWrite rho b\<rbrakk>
+           \<Longrightarrow> (a,b) \<in> singleorderdep T rho sb"
+| acqRelUpFence1 : "\<lbrakk> (a,b) \<in> trancl sb; isRealFence rho b;
+                            atLeastAcqRel rho b; isMemOp rho a\<rbrakk>
+           \<Longrightarrow> (a,b) \<in> singleorderdep T rho sb"
+| acqRelUpFence2 : "\<lbrakk> (a,b) \<in> trancl sb; isRealFence rho a;
+                            atLeastAcqRel rho a; isMemOp rho b\<rbrakk>
+           \<Longrightarrow> (a,b) \<in> singleorderdep T rho sb"
 
 
-(* define available after relation, it is a combination of all single thread dependency. *)
-inductive_set af :: "time_type set \<Rightarrow> (time_type \<Rightarrow> ('tid \<times> aid_type \<times>
+(* define the true program order relation,
+    it is a combination of all single thread dependency. *)
+inductive_set po :: "time_type set \<Rightarrow> (time_type \<Rightarrow> ('tid \<times> aid_type \<times>
                    (aid_type, 'val, loc_type, 'lock, 'name, 'callID) action) option) \<Rightarrow>
-              (time_type \<times> time_type) set
+              (time_type \<times> time_type) set \<Rightarrow> (time_type \<times> time_type) set
           \<Rightarrow> (time_type \<times> time_type) set"
-  for E :: "time_type set"
+  for T :: "time_type set"
     and rho :: "(time_type \<Rightarrow> ('tid \<times> aid_type \<times>
                    (aid_type, 'val, loc_type, 'lock, 'name, 'callID) action) option)"
-    and sb :: "(time_type \<times> time_type) set" where
- callRule : "(a,b) \<in> calldep E rho sb \<Longrightarrow> (a,b) \<in> af E rho sb"
-| controlRule : "(a,b) \<in> controldep E rho sb \<Longrightarrow> (a,b) \<in> af E rho sb"
-| dataRule : "(a,b) \<in> datadep E rho sb \<Longrightarrow> (a,b) \<in> af E rho sb"
-| volatileRule : "(a,b) \<in> volatileDep E rho sb \<Longrightarrow> (a,b) \<in> af E rho sb"
-| singleOrderRule : "(a,b) \<in> singleorderdep E rho sb \<Longrightarrow> (a,b) \<in> af E rho sb"
+    and sb :: "(time_type \<times> time_type) set"
+    and dd :: "(time_type \<times> time_type) set" where
+ callRule : "(a,b) \<in> calldep T rho sb \<Longrightarrow> (a,b) \<in> po T rho sb dd"
+| controlRule : "(a,b) \<in> controldep T rho sb \<Longrightarrow> (a,b) \<in> po T rho sb dd"
+| dataRule : "(a,b) \<in> dd \<Longrightarrow> (a,b) \<in> po T rho sb dd"
+| volatileRule : "(a,b) \<in> volatileDep T rho sb \<Longrightarrow> (a,b) \<in> po T rho sb dd"
+| singleOrderRule : "(a,b) \<in> singleorderdep T rho sb \<Longrightarrow> (a,b) \<in> po T rho sb dd"
+
+(* define a program order family (pos) as the transitive closure all po for all threads *)
+definition pos where
+"pos Tid T rho sbs dds = trancl (\<Union> tid \<in> Tid . po T rho (the (sbs tid)) (the (dds tid)))"
 
 (* a complete set for af, every dependency has an clear edge from one event to the other,
    these edges can act as an indication of which event should happen early than another event.
    if there is no edges between two events, it means that either one can happen early, so 
    it essentially means that there are two edges connecting this two. 
-   this process tries to add all two edges on no connected events. *)
+   this process tries to add all two edges on no connected events. 
 inductive_set completeAf :: "time_type set \<Rightarrow> (time_type \<Rightarrow> ('tid \<times> aid_type \<times>
                    (aid_type, 'val, loc_type, 'lock, 'name, 'callID) action) option) \<Rightarrow>
               (time_type \<times> time_type) set
@@ -584,8 +664,9 @@ completeLeft : "\<lbrakk> \<not> (a,b) \<in> trancl (af E rho sb); \<not> (b,a) 
              \<Longrightarrow> (a,b) \<in> completeAf E rho sb"
 | completeRight : "\<lbrakk> \<not> (a,b) \<in> trancl (af E rho sb); \<not> (b,a) \<in> trancl (af E rho sb) \<rbrakk>
              \<Longrightarrow> (b,a) \<in> completeAf E rho sb"
+*)
 
-(* get a set of initial state, where an execution can start with such time *)
+(* get a set of initial state, where an execution can start with such time 
 inductive_set initialStates :: "time_type set \<Rightarrow> (time_type \<Rightarrow> ('tid \<times> aid_type \<times>
                    (aid_type, 'val, loc_type, 'lock, 'name, 'callID) action) option) \<Rightarrow>
               (time_type \<times> time_type) set
@@ -616,149 +697,339 @@ definition isAllowedSingleExecution :: "time_type set \<Rightarrow> (time_type \
    (case allowedSingleExecutionSet E rho po of (init,R)
              \<Rightarrow> (the (getLeast E) \<in> init
                  \<and> allowedExecutionInductive (the (getLeast E), E - {the (getLeast E)}, R))))"
+*)
+
+(* defining an allowed execution in each single thread
+     by checking if there is an edge from a later time point to a earlier time point*)
+definition isAllowedSingleExecution :: "time_type set \<Rightarrow> (time_type \<Rightarrow> ('tid \<times> aid_type \<times>
+                   (aid_type, 'val, loc_type, 'lock, 'name, 'callID) action) option) \<Rightarrow>
+              (time_type \<times> time_type) set \<Rightarrow> (time_type \<times> time_type) set \<Rightarrow> bool" where
+"isAllowedSingleExecution T rho sb dd = (\<forall> a b . (a,b) \<in> po T rho sb dd \<longrightarrow> a < b)"
 
 fun selectTimeByTid where
-"selectTimeByTid tid E rho = {t . t \<in> E \<and> (\<exists> tid' aid ac . rho t = Some (tid',aid,ac) \<and> tid = tid')}"
+"selectTimeByTid tid T rho = {t . t \<in> T \<and> (\<exists> tid' aid ac . rho t = Some (tid',aid,ac) \<and> tid = tid')}"
 
-(* assume that rho satisfy the rho assumption *)
+(* the predicate for each thread in the tid-set to satisfy the allowed execution predicate above. *)
 definition satE :: "'tid set \<Rightarrow>
           time_type set \<Rightarrow> (time_type \<Rightarrow> ('tid \<times> aid_type \<times>
                    (aid_type, 'val, loc_type, 'lock, 'name, 'callID) action) option) \<Rightarrow>
-            ('tid \<Rightarrow> (time_type \<times> time_type) set option) \<Rightarrow> bool" where
-"satE Tid E rho pos = (\<forall> tid \<in> Tid . (\<forall> po . (pos tid) = Some po \<and> sbAllAssumptions po rho \<longrightarrow>
-                   isAllowedSingleExecution (selectTimeByTid tid E rho) rho (the (pos tid))))"
+            ('tid \<Rightarrow> (time_type \<times> time_type) set option)
+      \<Rightarrow> ('tid \<Rightarrow> (time_type \<times> time_type) set option) \<Rightarrow> bool" where
+"satE Tid T rho sbs dds = (\<forall> tid \<in> Tid . 
+                   isAllowedSingleExecution (selectTimeByTid tid T rho) rho (the (sbs tid)) (the (dds tid)))"
 
+(*
 definition localTimes where
 "localTimes ts f tid = {x . x \<in> ts \<and> (\<exists> h . f x = Some (tid, h))}"
+*)
 
-(* defining seqcst fence in the middle of two points *)
+(* Here, we start the definition of multi-threaded behaviors in ATRCM.
+   Basically, it defines two things. First, it defines the global total order of
+   SC atomics. Second, it defines a multi-threaded memory communication scheduler. *)
+(* defining the existence of a seqcst fence in the middle of two points *)
 definition seqFenceInMid where
-"seqFenceInMid T rho a b = (\<exists> t .
-                        t \<in> T \<and> a < t \<and> t < b \<and> isSeqFence (rho t))"
+"seqFenceInMid T rho a b = (\<exists> t . t \<in> T \<and> a < t \<and> t < b \<and> isSeqFence rho t)"
 
+(* defining the existence of a seqcst read in the middle of two points *)
 definition seqReadInMid where
-"seqReadInMid T rho a b x = (\<exists> t .
-                        t \<in> T \<and> a < t \<and> t < b \<and> isPureReadInTuple (rho t)
-                        \<and> isSeqAtomicInTuple (rho t) \<and> getLocInTuple (rho t) = Some x)"
+"seqReadInMid T rho a b x = (\<exists> t . t \<in> T \<and> a < t \<and> t < b \<and> isSeqRead rho t \<and> getLoc rho t = Some x)"
 
-definition isSeqRead where
-"isSeqRead rho a = (isPureReadInTuple (rho a) \<and> isSeqAtomicInTuple (rho a))"
+(* check if a non-atomic write is the final one in its group,
+             if so, then it is able to be read by another time point in rf *)
+definition isFinalNWrite where
+"isFinalNWrite rho t = (case rho t of Some (x,y,NWrite vol v loc aid i n) \<Rightarrow> i = n
+                                          | _ \<Rightarrow> False)"
 
-(* defining a write with the same location in the middle of two points *)
+(* defining the existence of a write with the same location in the middle of two points *)
 definition writeInMid where
 "writeInMid T rho a b loc = (\<exists> t .
-                        t \<in> T \<and> a < t \<and> t < b \<and> isTheLocInTuple (rho t) loc \<and> isWriteInTuple (rho t))"
+                        t \<in> T \<and> a < t \<and> t < b \<and> isTheLoc rho t loc \<and>
+            ((isWrite rho t \<and> isAtomic rho t) \<or>
+            (isWrite rho t \<and> \<not> isAtomic rho t \<and> isFinalNWrite rho t)))"
 
-(* defining a write with the same location in the middle of two points *)
+(* defining the existence of a write with the same location in the middle of two points *)
 definition sameThreadWriteInMid where
 "sameThreadWriteInMid T rho a b loc = (\<exists> t .
-                        t \<in> T \<and> a < t \<and> t < b \<and> isTheLocInTuple (rho t) loc \<and> isWriteInTuple (rho t)
+                        t \<in> T \<and> a < t \<and> t < b \<and> isTheLoc rho t loc \<and>
+            ((isWrite rho t \<and> isAtomic rho t) \<or>
+            (isWrite rho t \<and> \<not> isAtomic rho t \<and> isFinalNWrite rho t))
                           \<and> sameThread rho t b)"
 
-(* starting defining dependency crossing different threads 
-   we first define cw relation. cw relation is basically rf + seq fence relation.
-   In the model, the seq fence sychronizes all memory values for all locations.
-   So, a read from a write crossing a seq fence can be viewed as a read from a seq-fence, and 
-       a seq-fence from a write *)
+(* tr collects all write-read pairs in a thread that does not appear in rf*)
+inductive_set tr ::"time_type set \<Rightarrow> (time_type \<Rightarrow> ('tid \<times> aid_type \<times>
+                   (aid_type, 'val, loc_type, 'lock, 'name, 'callID) action) option) \<Rightarrow>
+              (time_type \<times> time_type) set
+          \<Rightarrow> (time_type \<times> loc_type \<times> time_type) set"
+  for T :: "time_type set"
+    and rho :: "(time_type \<Rightarrow> ('tid \<times> aid_type \<times>
+                   (aid_type, 'val, loc_type, 'lock, 'name, 'callID) action) option)"
+    and rf :: "(time_type \<times> time_type) set" where
+trEmpty : "\<lbrakk> \<not> sameThreadWriteInMid T rho a b x; isRead rho b; getLoc rho b = Some x;
+                       a = 0; b \<in> T\<rbrakk> \<Longrightarrow> (a,x,b) \<in> tr T rho rf"
+| trGet : "\<lbrakk> \<not> sameThreadWriteInMid E rho a b x; isWrite rho a;isRead rho b;
+             getLoc rho b = Some x;sameLoc rho a b;sameThread rho a b; b \<in> T \<rbrakk> \<Longrightarrow> (a,x,b) \<in> tr T rho rf"
+
+lemma trZero : "\<lbrakk> rhoAssumption T \<rho>; a \<in> T; b \<in> T;
+       wellformedTime T \<rho> rf ; wellformedRF T \<rho> rf ;(a,x,b) \<in> tr T \<rho> rf\<rbrakk>
+         \<Longrightarrow> a \<noteq> 0"
+  apply (erule tr.cases)
+   apply (simp add: wellformedTime_def rhoAssumption_def wellformedRF_def,clarsimp)
+  apply (simp add: wellformedTime_def rhoAssumption_def wellformedRF_def,clarsimp)
+  apply (subgoal_tac "a \<in> T \<and> 0 \<notin> T \<longrightarrow> a \<noteq> 0")
+   apply simp
+  by auto
+
+lemma trReadInSet : "(a,x,b) \<in> tr T \<rho> rf \<Longrightarrow> b \<in> T"
+  apply (erule tr.cases)
+  by auto
+
+lemma isWriteInTR : "\<lbrakk> rhoAssumption T \<rho>; a \<in> T; b \<in> T;
+       wellformedTime T \<rho> rf ; wellformedRF T \<rho> rf ;(a,x,b) \<in> tr T \<rho> rf\<rbrakk>
+          \<Longrightarrow> isWrite \<rho> a"
+  apply (erule tr.cases)
+  by (simp add: wellformedTime_def rhoAssumption_def wellformedRF_def,clarsimp)
+
+lemma sameLocInTR : "\<lbrakk> rhoAssumption T \<rho>; a \<in> T; b \<in> T;
+       wellformedTime T \<rho> rf ; wellformedRF T \<rho> rf ;(a,x,b) \<in> tr T \<rho> rf\<rbrakk>
+          \<Longrightarrow> sameLoc \<rho> a b"
+  apply (erule tr.cases)
+  by (simp add: wellformedTime_def rhoAssumption_def wellformedRF_def,clarsimp)
+
+lemma locXInTR : "\<lbrakk> rhoAssumption T \<rho>; a \<in> T; b \<in> T;
+       wellformedTime T \<rho> rf ; wellformedRF T \<rho> rf ;(a,x,b) \<in> tr T \<rho> rf\<rbrakk>
+          \<Longrightarrow> getLoc \<rho> b = Some x"
+  apply (erule tr.cases)
+  by (simp add: wellformedTime_def rhoAssumption_def wellformedRF_def,clarsimp)
+
+(* fullRf = rf \<union> tr *)
+definition fullRf where
+"fullRf T rho rf = ({(a,x,b) . (a,b) \<in> rf \<and> getLoc rho a = Some x} \<union> tr T rho rf)"
+
+lemma fullRfReadInSet : "\<lbrakk> rhoAssumption T \<rho>;
+       wellformedTime T \<rho> rf ; wellformedRF T \<rho> rf ; (a,x,b) \<in> fullRf T \<rho> rf\<rbrakk> 
+            \<Longrightarrow> b \<in> T"
+  apply (simp add: fullRf_def)
+  apply (case_tac "(a, x, b) \<in> tr T \<rho> rf",clarsimp)
+   apply (simp add: trReadInSet)
+  apply clarsimp
+  by (simp add: wellformedTime_def wellformedRF_def rhoAssumption_def)
+
+lemma isWriteInFullRf : "\<lbrakk> rhoAssumption T \<rho>; a \<in> T; b \<in> T;
+       wellformedTime T \<rho> rf ; wellformedRF T \<rho> rf ; (a,x,b) \<in> fullRf T \<rho> rf\<rbrakk> 
+            \<Longrightarrow> isWrite \<rho> a"
+  apply (simp add: fullRf_def)
+  apply (case_tac "\<rho> a")
+   apply clarsimp
+   apply (simp add: wellformedTime_def wellformedRF_def rhoAssumption_def,clarsimp)
+  apply (subgoal_tac "a \<in> T \<and> T \<subseteq> dom \<rho> \<longrightarrow> \<rho> a \<noteq> None")
+    apply clarsimp
+  apply blast
+  apply (case_tac "(a, x, b) \<in> tr T \<rho> rf",clarsimp)
+   apply (subgoal_tac " isWrite \<rho> a")
+    apply simp
+   apply (erule_tac a = a and x = x and b = b and T = T and \<rho> = \<rho> and rf = rf in isWriteInTR)
+  apply clarsimp+
+  apply (simp add: wellformedTime_def wellformedRF_def rhoAssumption_def)
+  apply (erule_tac x = "a" in allE)
+  apply (erule_tac x = "b" in allE)
+  by auto
+
+lemma sameLocInFullRf : "\<lbrakk> rhoAssumption T \<rho>; a \<in> T; b \<in> T;
+       wellformedTime T \<rho> rf ; wellformedRF T \<rho> rf ; (a,x,b) \<in> fullRf T \<rho> rf\<rbrakk> 
+            \<Longrightarrow> sameLoc \<rho> a b"
+  apply (simp add: fullRf_def)
+  apply (case_tac "\<rho> a")
+   apply clarsimp
+   apply (simp add: wellformedTime_def wellformedRF_def rhoAssumption_def,clarsimp)
+  apply (subgoal_tac "a \<in> T \<and> T \<subseteq> dom \<rho> \<longrightarrow> \<rho> a \<noteq> None")
+    apply clarsimp
+  apply blast
+  apply (case_tac "(a, x, b) \<in> tr T \<rho> rf",clarsimp)
+   apply (subgoal_tac "sameLoc \<rho> a b")
+    apply simp
+   apply (erule_tac a = a and x = x and b = b and T = T and \<rho> = \<rho> and rf = rf in sameLocInTR)
+  apply clarsimp+
+  apply (simp add: wellformedTime_def wellformedRF_def rhoAssumption_def)
+  apply (erule_tac x = "a" in allE)
+  apply (erule_tac x = "b" in allE)
+  by auto
+
+lemma locXInFullRf : "\<lbrakk> rhoAssumption T \<rho>; a \<in> T; b \<in> T;
+       wellformedTime T \<rho> rf ; wellformedRF T \<rho> rf ; (a,x,b) \<in> fullRf T \<rho> rf\<rbrakk> 
+            \<Longrightarrow> getLoc \<rho> b = Some x"
+  apply (simp add: fullRf_def)
+  apply (case_tac "\<rho> b")
+   apply clarsimp
+   apply (simp add: wellformedTime_def wellformedRF_def rhoAssumption_def,clarsimp)
+  apply (subgoal_tac "b \<in> T \<and> T \<subseteq> dom \<rho> \<longrightarrow> \<rho> b \<noteq> None")
+    apply clarsimp
+  apply blast
+  apply (case_tac "(a, x, b) \<in> tr T \<rho> rf",clarsimp)
+   apply (subgoal_tac "getLoc \<rho> b = Some x")
+    apply simp
+   apply (erule_tac a = a and x = x and b = b and T = T and \<rho> = \<rho> and rf = rf in locXInTR)
+  apply clarsimp+
+  apply (simp add: wellformedRF_def,clarsimp)
+  apply (erule_tac x = "a" in allE)
+  apply (erule_tac x = "a" in allE)
+  apply (erule_tac x = "b" in allE)
+  apply (erule_tac x = "b" in allE)
+  apply clarsimp
+  apply (case_tac "\<rho> a")
+   apply clarsimp
+  apply clarsimp
+  apply (case_tac "acLoc ba")
+   apply clarsimp
+  apply clarsimp
+  apply (case_tac "x = ad")
+  by clarsimp+
+
+lemma sameLocTwoInFullRf: "\<lbrakk> rhoAssumption T \<rho>; s \<in> T; t \<in> T;
+       wellformedTime T \<rho> rf ; wellformedRF T \<rho> rf ; (s,x,a) \<in> fullRf T \<rho> rf; (t,x,b) \<in> fullRf T \<rho> rf\<rbrakk> 
+            \<Longrightarrow> sameLoc \<rho> s t"
+  apply (subgoal_tac "a \<in> T")
+   prefer 2
+  apply (simp add: fullRfReadInSet)
+  apply (subgoal_tac "b \<in> T")
+   prefer 2
+  apply (simp add: fullRfReadInSet)
+  apply (subgoal_tac "getLoc \<rho> a = Some x")
+   prefer 2
+   apply (erule_tac T = T and \<rho> = \<rho> and a = s and b = a and x = x and rf = rf in locXInFullRf)
+  apply (simp,simp,simp,simp,simp)
+  apply (subgoal_tac "getLoc \<rho> b = Some x")
+   prefer 2
+   apply (erule_tac T = T and \<rho> = \<rho> and a = t and b = b and x = x and rf = rf in locXInFullRf)
+  apply (simp,simp,simp,simp,simp)
+  apply (subgoal_tac "sameLoc \<rho> s a")
+   prefer 2
+  thm sameLocInFullRf
+  apply (erule_tac T = T and \<rho> = \<rho> and a = s and b = a and x = x and rf = rf in sameLocInFullRf)
+  apply (simp,simp,simp,simp,simp)
+  apply (subgoal_tac "sameLoc \<rho> t b")
+  prefer 2
+   apply (erule_tac T = T and \<rho> = \<rho> and a = t and b = b and x = x and rf = rf in sameLocInFullRf)
+       apply (simp,simp,simp,simp,simp)
+  apply auto
+  apply (case_tac "\<rho> a")
+   apply clarsimp
+  apply (case_tac "\<rho> b")
+   apply clarsimp
+  apply (case_tac "\<rho> s")
+   apply clarsimp
+  apply (case_tac "\<rho> t")
+   apply clarsimp+
+  apply (case_tac "acLoc bb")
+   apply (simp add: wellformedTime_def wellformedRF_def rhoAssumption_def,clarsimp)
+  apply (case_tac "acLoc bc")
+   apply (simp add: wellformedTime_def wellformedRF_def rhoAssumption_def,clarsimp)
+  apply (case_tac "ah = x")
+   apply clarsimp
+  apply (case_tac "ai = x")
+  by clarsimp+
+
+definition full_rf where
+"full_rf T rho rf = { (a,b) . \<exists> x . (a,x,b) \<in> (fullRf T rho rf) }"
+
+(* sr is to define write-read pairs for a seqcst-read/seqcst-fence.
+   we view the seqcst fence as a universal read op to observe a value for a location for every location *)
 inductive_set sr :: "time_type set \<Rightarrow> (time_type \<Rightarrow> ('tid \<times> aid_type \<times>
                    (aid_type, 'val, loc_type, 'lock, 'name, 'callID) action) option) \<Rightarrow>
               (time_type \<times> time_type) set
           \<Rightarrow> (time_type \<times> loc_type \<times> time_type) set"
-  for E :: "time_type set"
+  for T :: "time_type set"
     and rho :: "(time_type \<Rightarrow> ('tid \<times> aid_type \<times>
                    (aid_type, 'val, loc_type, 'lock, 'name, 'callID) action) option)"
     and rf :: "(time_type \<times> time_type) set" where
-  fromSeqFence : "\<lbrakk> a < b; isWriteInTuple (rho a);  isSeqFence (rho b);
-                     getLocInTuple (rho a) = Some x; \<not> seqFenceInMid E rho a b;
-                   \<not> writeInMid E rho a b x; \<not> seqReadInMid E rho a b x\<rbrakk> \<Longrightarrow> (a,x,b) \<in> sr E rho rf"
-| seqFenceInduct : "\<lbrakk> (a,x,b') \<in> sr E rho rf; b' < b; b \<in> E; isSeqFence (rho b);
-                       isWriteInTuple (rho a); getLocInTuple (rho a) = Some x;
-                       \<not> seqFenceInMid E rho b' b; \<not> writeInMid E rho b' b x; \<not> seqReadInMid E rho b' b x\<rbrakk>
-                          \<Longrightarrow> (a,x,b) \<in> sr E rho rf"
-| seqFenceEmpty : "\<lbrakk> isSeqFence (rho b);
-                      \<not> seqFenceInMid E rho 0 b;
-                   \<not> writeInMid E rho 0 b x; \<not> seqReadInMid E rho 0 b x\<rbrakk>
-                          \<Longrightarrow> (0,x,b) \<in> sr E rho rf"
+  fromSeqFence : "\<lbrakk> {a,b} \<subseteq> T; a < b; isWrite rho a;  isSeqFence rho b;
+                     getLoc rho a = Some x; \<not> seqFenceInMid T rho a b;
+                   \<not> writeInMid T rho a b x; \<not> seqReadInMid T rho a b x\<rbrakk> \<Longrightarrow> (a,x,b) \<in> sr T rho rf"
+| seqFenceInduct : "\<lbrakk> (a,x,b') \<in> sr T rho rf; b' < b; b \<in> T; isSeqFence rho b;
+                       isWrite rho a; getLoc rho a = Some x;
+                       \<not> seqFenceInMid T rho b' b; \<not> writeInMid T rho b' b x; \<not> seqReadInMid T rho b' b x\<rbrakk>
+                          \<Longrightarrow> (a,x,b) \<in> sr T rho rf"
+|  fromSeqRead : "\<lbrakk> {a,b} \<subseteq> T; a < b; isWrite rho a;  isSeqRead rho b;
+                     getLoc rho a = Some x; sameLoc rho a b; \<not> seqFenceInMid T rho a b;
+                   \<not> writeInMid T rho a b x; \<not> seqReadInMid T rho a b x\<rbrakk> \<Longrightarrow> (a,x,b) \<in> sr T rho rf"
+| seqFenceInductRead : "\<lbrakk> (a,x,b') \<in> sr T rho rf; b' < b; b \<in> T; isSeqRead rho b;
+                       isWrite rho a; getLoc rho a = Some x; sameLoc rho a b;
+                       \<not> seqFenceInMid T rho b' b; \<not> writeInMid T rho b' b x; \<not> seqReadInMid T rho b' b x\<rbrakk>
+                          \<Longrightarrow> (a,x,b) \<in> sr T rho rf"
+| seqFenceEmpty : "\<lbrakk> isSeqFence rho b;
+                      \<not> seqFenceInMid T rho 0 b;
+                   \<not> writeInMid E rho 0 b x; \<not> seqReadInMid T rho 0 b x\<rbrakk>
+                          \<Longrightarrow> (0,x,b) \<in> sr T rho rf"
 | seqReadEmpty : "\<lbrakk>  isSeqRead rho b;
-                     getLocInTuple (rho b) = Some x; \<not> seqFenceInMid E rho 0 b;
-                   \<not> writeInMid E rho 0 b x; \<not> seqReadInMid E rho 0 b x\<rbrakk>
-                          \<Longrightarrow> (0,x,b) \<in> sr E rho rf"
-| fromSeqRead : "\<lbrakk> a < b; isWriteInTuple (rho a);  isSeqRead rho b; sameLocInTuple rho a b;
-                     getLocInTuple (rho a) = Some x; \<not> seqFenceInMid E rho a b;
-                   \<not> writeInMid E rho a b x; \<not> seqReadInMid E rho a b x\<rbrakk> \<Longrightarrow> (a,x,b) \<in> sr E rho rf"
-| seqReadInduct : "\<lbrakk> (a,x,b') \<in> sr E rho rf; b' < b; b \<in> E; isSeqRead rho b;
-                       isWriteInTuple (rho a); getLocInTuple (rho a) = Some x; sameLocInTuple rho a b;
-                       \<not> seqFenceInMid E rho b' b; \<not> writeInMid E rho b' b x; \<not> seqReadInMid E rho b' b x\<rbrakk>
-                          \<Longrightarrow> (a,x,b) \<in> sr E rho rf"
+                     getLoc rho b = Some x; \<not> seqFenceInMid T rho 0 b;
+                   \<not> writeInMid T rho 0 b x; \<not> seqReadInMid T rho 0 b x\<rbrakk>
+                          \<Longrightarrow> (0,x,b) \<in> sr T rho rf"
 
-
-inductive_set cw :: "time_type set \<Rightarrow> (time_type \<Rightarrow> ('tid \<times> aid_type \<times>
-                   (aid_type, 'val, loc_type, 'lock, 'name, 'callID) action) option) \<Rightarrow>
-              (time_type \<times> time_type) set
-          \<Rightarrow> (time_type \<times> loc_type \<times> time_type) set"
-  for E :: "time_type set"
-    and rho :: "(time_type \<Rightarrow> ('tid \<times> aid_type \<times>
-                   (aid_type, 'val, loc_type, 'lock, 'name, 'callID) action) option)"
-    and rf :: "(time_type \<times> time_type) set" where
- inrf : "\<lbrakk> (a,b) \<in> rf ; getLocInTuple (rho a) = Some x\<rbrakk> \<Longrightarrow> (a,x,b) \<in> cw E rho rf"
-| insr : "\<lbrakk> (\<forall> t . (t ,b) \<notin> rf) ; (a,x,b') \<in> sr E rho rf; b' < b; b \<in> E;
-               isReadInTuple (rho b); \<not> sameThreadWriteInMid E rho b' b x\<rbrakk> \<Longrightarrow> (a,x,b) \<in> cw E rho rf"
-| inSingle : "\<lbrakk>(\<forall> t . (t ,b) \<notin> rf) ; a  < b; b \<in> E; a \<in> E;
-                isWriteInTuple (rho a); sameThread rho a b;
-               isReadInTuple (rho b); \<not> seqFenceInMid E rho a b; \<not> seqReadInMid E rho a b x;
-               \<not> sameThreadWriteInMid E rho a b x\<rbrakk>
-                          \<Longrightarrow> (a,x,b) \<in> cw E rho rf"
-| inempty : "\<lbrakk>(\<forall> t . (t ,b) \<notin> rf) ; b \<in> E;
-               isReadInTuple (rho b); \<not> seqFenceInMid E rho 0 b; \<not> seqReadInMid E rho 0 b x;
-               \<not> sameThreadWriteInMid E rho 0 b x\<rbrakk>
-                          \<Longrightarrow> (0,x,b) \<in> cw E rho rf"
-
+(* cw is tr \<union> sr \<union> rf *)
+definition cw where
+"cw E rho rf = ({(a,x,b) . (a,b) \<in> rf \<and> getLoc rho a = Some x} \<union> tr E rho rf \<union> sr E rho rf)"
 
 (*define cocw relation meaning that a write-read relation that cannot appear in an execution of a rf *)
 
-(* if there is a sequence fence or sequence read-write in the middle with the same location *)
+(* check the unqulified full-rf relations on seqcst atomics. 
+    if there is a sequence fence or sequence read-write in the middle with the same location *)
 inductive_set seqCocw :: "time_type set \<Rightarrow> (time_type \<Rightarrow> ('tid \<times> aid_type \<times>
                    (aid_type, 'val, loc_type, 'lock, 'name, 'callID) action) option) \<Rightarrow>
               (time_type \<times> time_type) set
           \<Rightarrow> (time_type \<times> time_type) set"
-  for E :: "time_type set"
+  for T :: "time_type set"
     and rho :: "(time_type \<Rightarrow> ('tid \<times> aid_type \<times>
                    (aid_type, 'val, loc_type, 'lock, 'name, 'callID) action) option)"
     and rf :: "(time_type \<times> time_type) set" where
- seqCocw1 : "\<lbrakk>(a,b) \<in> rf ; rho t = Some (tid,aid, Fence SeqCst); getLocInTuple (rho a) = Some x;
-                (a,x,t) \<notin> cw E rho rf; t > a ; t < b\<rbrakk> 
-                    \<Longrightarrow> (a,b) \<in> seqCocw E rho rf"
-| seqCocw2 : "\<lbrakk>(a,b) \<in> rf ; rho t = Some (tid,aid, ac); getLocInTuple (rho a) = Some x;
-                isSeqAtomic ac; (a,x,t) \<notin> cw E rho rf; t > a ; t < b\<rbrakk> 
-                    \<Longrightarrow> (a,b) \<in> seqCocw E rho rf"
-| seqCocw3 : "\<lbrakk>(a,b) \<in> rf ; rho t = Some (tid,aid, ac); getLocInTuple (rho a) = Some x;
-                isSeqAtomic ac; isWrite ac; t > a ; t < b\<rbrakk> 
-                    \<Longrightarrow> (a,b) \<in> seqCocw E rho rf"
+ seqCocwWrite : "\<lbrakk>(a,x,b) \<in> fullRf T rho rf ; t \<in> T; a < t; t < b;
+                     isWrite rho t; isSeqAtomic rho t; getLoc rho t = Some x \<rbrakk> 
+                    \<Longrightarrow> (a,b) \<in> seqCocw T rho rf"
+| seqCocwFence : "\<lbrakk>(a,x,b) \<in> fullRf T rho rf ; t \<in> T; a < t; t < b; isSeqFence rho t;
+                      (a,x,t) \<notin> cw T rho rf\<rbrakk> 
+                    \<Longrightarrow> (a,b) \<in> seqCocw T rho rf"
+| seqCocwRead : "\<lbrakk>(a,x,b) \<in> fullRf T rho rf ; t \<in> T; a < t; t < b; isSeqRead rho t;
+                        sameLoc rho a t; (a,x,t) \<notin> cw T rho rf\<rbrakk> 
+                    \<Longrightarrow> (a,b) \<in> seqCocw T rho rf"
+| seqCocwSame : "\<lbrakk>(a,x,b) \<in> fullRf T rho rf ; t \<in> T; a \<noteq> t; (t,x,b) \<in> cw T rho rf\<rbrakk> 
+                    \<Longrightarrow> (a,b) \<in> seqCocw T rho rf"
 
 (* in this model, since we have single thread non-determinsm of event moving,
    the cross thread model can be defined very simply. reads in a thread receiving 
      writes from another thread are in a FIFO order, the crossCocw is to rule out un-FIFO order read-writes.*)
-inductive_set crossCocw :: "time_type set \<Rightarrow> (time_type \<Rightarrow> ('tid \<times> aid_type \<times>
+inductive_set fifoCocw :: "time_type set \<Rightarrow> (time_type \<Rightarrow> ('tid \<times> aid_type \<times>
                    (aid_type, 'val, loc_type, 'lock, 'name, 'callID) action) option) \<Rightarrow>
               (time_type \<times> time_type) set
           \<Rightarrow> (time_type \<times> time_type) set"
-  for E :: "time_type set"
+  for T :: "time_type set"
     and rho :: "(time_type \<Rightarrow> ('tid \<times> aid_type \<times>
                    (aid_type, 'val, loc_type, 'lock, 'name, 'callID) action) option)"
     and rf :: "(time_type \<times> time_type) set" where
- crossCocw1 : "\<lbrakk>(a,x,b) \<in> cw E rho rf \<and>
-                 (\<exists> t t' . t \<in> E \<and> t' \<in> E \<and> t' < a \<and> b < t \<and> sameThread rho b t
-                     \<and> (t',x,t) \<in> cw E rho rf)\<rbrakk> 
-                    \<Longrightarrow> (a,b) \<in> crossCocw E rho rf"
-| crossCocw2 : "\<lbrakk>(a,x,b) \<in> cw E rho rf \<and>
-                 (\<exists> t t' . t \<in> E \<and> t' \<in> E \<and> a < t' \<and> t < b \<and> sameThread rho b t
-                     \<and> (t',x,t) \<in> cw E rho rf)\<rbrakk> 
-                    \<Longrightarrow> (a,b) \<in> crossCocw E rho rf"
+nonfifoOrder : "\<lbrakk>(a,x,b) \<in> fullRf T rho rf ; (c,y,d) \<in> fullRf T rho rf; a > c ; d > b\<rbrakk> 
+                    \<Longrightarrow> (a,b) \<in> fifoCocw T rho rf"
 
+inductive_set coherenceCocw :: "time_type set \<Rightarrow> (time_type \<Rightarrow> ('tid \<times> aid_type \<times>
+                   (aid_type, 'val, loc_type, 'lock, 'name, 'callID) action) option) \<Rightarrow>
+              (time_type \<times> time_type) set
+          \<Rightarrow> (time_type \<times> time_type) set"
+  for T :: "time_type set"
+    and rho :: "(time_type \<Rightarrow> ('tid \<times> aid_type \<times>
+                   (aid_type, 'val, loc_type, 'lock, 'name, 'callID) action) option)"
+    and rf :: "(time_type \<times> time_type) set" where
+ coherenceCocw1 : "\<lbrakk>(a,x,b) \<in> fullRf T rho rf ; (s,x,t) \<in> fullRf T rho rf;
+                         a < s ; b > t; sameThread rho b t\<rbrakk> 
+                    \<Longrightarrow> (a,b) \<in> coherenceCocw T rho rf"
+| coherenceCocw2 : "\<lbrakk>(a,x,b) \<in> fullRf T rho rf ; (s,x,t) \<in> fullRf T rho rf;
+                         a < s ; b > t; sameThread rho b t; sameThread rho a s\<rbrakk> 
+                    \<Longrightarrow> (a,b) \<in> coherenceCocw T rho rf"
+
+(* cocw for fifo order, cocw must be empty *)
+definition cocwFIFO where
+"cocwFIFO T rho rf = seqCocw T rho rf \<union> fifoCocw T rho rf"
+
+(* cocw for coherence order, cocw must be empty *)
 definition cocw where
-"cocw E rho rf = seqCocw E rho rf \<union> crossCocw E rho rf"
+"cocw T rho rf = seqCocw T rho rf \<union> coherenceCocw T rho rf"
 
-(* defining memory loc creation property. Every mem-op must happen after its loc creates. *)
+(* defining memory loc creation property. Every mem-op must happen after its loc creates. 
 inductive_set createPro :: "time_type set \<Rightarrow> (time_type \<Rightarrow> ('tid \<times> aid_type \<times>
                    (aid_type, 'val, loc_type, 'lock, 'name, 'callID) action) option)
           \<Rightarrow> (time_type \<times> time_type) set"
@@ -766,7 +1037,7 @@ inductive_set createPro :: "time_type set \<Rightarrow> (time_type \<Rightarrow>
     and rho :: "(time_type \<Rightarrow> ('tid \<times> aid_type \<times>
                    (aid_type, 'val, loc_type, 'lock, 'name, 'callID) action) option)" where
  createBeforeUse : "\<lbrakk>a \<in> E; b \<in> E; a < b;
-                       sameLocInTuple rho a b;  isCreate (rho a); \<not> isCreate (rho b)\<rbrakk> 
+                       sameLoc rho a b;  isCreate rho a; \<not> isCreate rho b\<rbrakk> 
                     \<Longrightarrow> (a,b) \<in> createPro E rho"
 
 inductive_set freePro :: "time_type set \<Rightarrow> (time_type \<Rightarrow> ('tid \<times> aid_type \<times>
@@ -776,18 +1047,52 @@ inductive_set freePro :: "time_type set \<Rightarrow> (time_type \<Rightarrow> (
     and rho :: "(time_type \<Rightarrow> ('tid \<times> aid_type \<times>
                    (aid_type, 'val, loc_type, 'lock, 'name, 'callID) action) option)" where
  notUseAfterFree : "\<lbrakk>a \<in> E; b \<in> E; a < b;
-                       sameLocInTuple rho a b;  isFree (rho b); \<not> isFree (rho a)\<rbrakk> 
+                       sameLoc rho a b;  isFree rho b; \<not> isFree rho a\<rbrakk> 
                     \<Longrightarrow> (a,b) \<in> freePro E rho"
-
+*)
+(* the predicate is useful in proving all executions generated from a program. 
+   to check if there is potential write to a location before the location exists. 
 definition satCreationAndFree where
-"satCreationAndFree T rho = ((\<forall> a b . a \<in> T \<and> b \<in> T \<and> sameLocInTuple rho a b \<and> isCreate (rho a) 
+"satCreationAndFree T rho = ((\<forall> a b . a \<in> T \<and> b \<in> T \<and> sameLoc rho a b \<and> isCreate rho a
                            \<longrightarrow> (a,b) \<in> createPro T rho)
-                          \<and> (\<forall> a b . a \<in> T \<and> b \<in> T \<and> sameLocInTuple rho a b \<and> isFree (rho b) 
+                          \<and> (\<forall> a b . a \<in> T \<and> b \<in> T \<and> sameLoc rho a b \<and> isFree rho b 
                            \<longrightarrow> (a,b) \<in> freePro T rho))"
+*)
+(* an execution for FIFO order must sat the predicate *)
+definition satFIFO where
+"satFIFO Tid T rho sbs dds rf = (rhoAssumption T rho \<and> rfAllAssumption rf rho
+                           \<and> (satE Tid T rho sbs dds \<and> (cocwFIFO T rho rf = {})))"
 
+(* an execution for coherence order must sat the predicate *)
 definition sat where
-"sat Tid T rho po rf = (rhoAssumption rho \<and> rfAllAssumption rf rho
-                    \<longrightarrow> (satCreationAndFree T rho \<and> satE Tid T rho po \<and> (\<forall> (a,b) \<in> rf . (a,b) \<notin> cocw T rho rf)))"
+"sat Tid T rho sbs dds rf = (satE Tid T rho sbs dds \<and> (cocw T rho rf = {}))"
+
+lemma sat_le: 
+  fixes t1 t2 a b x
+  assumes sat1: "sat Tid T \<rho> sbs dds rf"
+      and FullRFa : "(t1,x,a) \<in> fullRf T \<rho> rf"
+      and FullRFb : "(t2,x,b) \<in> fullRf T \<rho> rf"
+      and AgtB: "a > b"
+      and sameThd : "sameThread \<rho> a b"
+    shows "t1 \<ge> t2"
+proof -
+  from sat1 
+  have COCW_empty: "cocw T \<rho> rf = {}"
+    by (simp add: sat_def)
+  from COCW_empty
+  have Coherence_empty: "coherenceCocw T \<rho> rf = {}"
+    by (simp add: cocw_def)
+  from  FullRFa and  FullRFb and AgtB and sameThd and coherenceCocw1
+  have B1: "t1 < t2 \<longrightarrow> (t1,a) \<in> coherenceCocw T \<rho> rf"
+    by (clarsimp )
+  from B1
+  have B2: "(t1,a) \<notin> coherenceCocw T \<rho> rf \<longrightarrow> t1 \<ge> t2"
+    by clarsimp
+  from B2 and Coherence_empty
+  show "t1 \<ge> t2"
+    by (simp add: B2 Coherence_empty)
+qed
+
 
 (* define locks model *)
 definition termInMid :: "time_type set \<Rightarrow> (time_type \<Rightarrow> ('tid \<times> aid_type \<times>
@@ -802,34 +1107,42 @@ definition termInSameTid :: "time_type set \<Rightarrow> (time_type \<Rightarrow
 "termInSameTid T rho a b e = (\<exists> t tid aid ac . t \<in> T \<and> a < t \<and> t < b
                      \<and> rho t = Some (tid,aid,ac) \<and> ac = e \<and> sameThread rho a t \<and> sameThread rho t b)"
 
+(* define the predicate for lock/unlock actions *)
 definition lockProp where
 "lockProp t l rho T = ((\<forall> t1 t2 . t1 \<in> T \<and> t2 \<in> T \<and> t < t1 \<and> t < t2 \<and> sameThread rho t t1 
-                            \<longrightarrow> \<not> hasAction (rho t1) (UnLock l) \<and> \<not> hasAction (rho t2) (Lock l))
-                         \<or> (\<exists> t' \<in> T . t < t' \<and> sameThread rho t t' \<and> hasAction (rho t') (UnLock l)
+                            \<longrightarrow> \<not> hasAction rho t1 (UnLock l) \<and> \<not> hasAction rho t2 (Lock l))
+                         \<or> (\<exists> t' \<in> T . t < t' \<and> sameThread rho t t' \<and> hasAction rho t' (UnLock l)
                              \<and> \<not> termInMid T rho t t' (Lock l) \<and> \<not> termInSameTid T rho t t' (UnLock l)))"
 
 definition locksProp where
-"locksProp T rho = (\<forall> t \<in> T . (\<forall> l \<in> locks . hasAction (rho t) (Lock l) \<longrightarrow> lockProp t l rho T))"
+"locksProp T rho = (\<forall> t \<in> T . (\<forall> l \<in> locks . hasAction rho t (Lock l) \<longrightarrow> lockProp t l rho T))"
 
 (* define a valid execution that needs to satisfy,
    an execution is (Tid, T, rho, sb, rf), and the validExecution predicate defines when an execution is valid.*)
+(* for FIFO execution *)
+definition validExecutionFIFO where
+"validExecutionFIFO Tid T rho sbs dds rf = 
+  (wellformedTime T rho rf \<and> wellformedTid Tid rho \<and> wellformedSB Tid T sbs \<and> wellformedDD Tid sbs dds
+   \<and> wellformedRF T rho rf \<and> rhoAssumption T rho \<and> rfAllAssumption rf rho
+   \<and> allSbAllAssumptions Tid sbs rho \<and> (locksProp T rho \<and> satFIFO Tid T rho sbs dds rf))"
 
+(* for coherence execution *)
 definition validExecution where
-"validExecution Tid T rho sb rf = 
-  (wellformedTime T rf rho \<and> wellformedTid Tid rho \<and> wellformedSB Tid T sb \<and>
-  (((\<forall> t \<in> Tid . (\<forall> (a,b) \<in> the (sb t) . a \<in> T \<and> b \<in> T))
-                \<and> (\<forall> (a,b) \<in> rf . a \<in> T \<and> b \<in> T) \<and> (\<forall> a \<in> T . rho a \<noteq> None)) 
-    \<longrightarrow> (locksProp T rho \<and> sat Tid T rho sb rf)))"
+"validExecution Tid T rho sbs dds rf = 
+  (wellformedTime T rho rf \<and> wellformedTid Tid rho \<and> wellformedSB Tid T sbs 
+  \<and> wellformedDD Tid sbs dds \<and> wellformedRF T rho rf \<and>
+   rhoAssumption T rho \<and> rfAllAssumption rf rho \<and> allSbAllAssumptions Tid sbs rho \<and>
+  (locksProp T rho \<and> sat Tid T rho sbs dds rf))"
 
 (* define race condition *)
 fun existOtherOp :: "time_type \<Rightarrow> loc_type
                \<Rightarrow> (aid_type, 'val, loc_type, 'lock, 'name, 'callID) action \<Rightarrow> bool" where
-"existOtherOp key loc (ARead vol v x y axl) = (if loc = x then True else False)"
-| "existOtherOp key loc (AWrite vol v x y axl) = (if loc = x then True else False)"
-| "existOtherOp key loc (RMW vol v x y axl) = (if loc = x then True else False)"
-| "existOtherOp key loc (NRead vol v x t na n axl) = (if key = t then False else
+"existOtherOp key loc (ARead vol v x y) = (if loc = x then True else False)"
+| "existOtherOp key loc (AWrite vol v x y) = (if loc = x then True else False)"
+| "existOtherOp key loc (RMW vol v x y) = (if loc = x then True else False)"
+| "existOtherOp key loc (NRead vol v x t na n) = (if key = t then False else
                                              (if loc = x then True else False))"
-| "existOtherOp key loc (NWrite vol v x t na n axl) = (if key = t then False else
+| "existOtherOp key loc (NWrite vol v x t na n) = (if key = t then False else
                                              (if loc = x then True else False))"
 | "existOtherOp key loc x = False"
 
@@ -845,8 +1158,9 @@ fun existOthers :: "time_type \<Rightarrow> loc_type
 "existOthers key loc rho T = (\<exists> t \<in> T . existOtherOpInTuple key loc (rho t))"
 
 fun raceDef where
-"raceDef T rho = (\<exists> t1 t2 tid aid1 aid2 v v' x t n axl vol . t1 \<in> T \<and> t2 \<in> T \<and> rho t1 = Some (tid,aid1, NRead vol v x t 1 n axl)
-                       \<and> rho t2 = Some (tid, aid2, NRead vol v' x t n n axl) 
+"raceDef T rho = (\<exists> t1 t2 tid aid1 aid2 v v' x t n vol . t1 \<in> T \<and> t2 \<in> T
+                       \<and> rho t1 = Some (tid,aid1, NRead vol v x t 1 n)
+                       \<and> rho t2 = Some (tid, aid2, NRead vol v' x t n n) 
                      \<longrightarrow> existOthers t x rho {h . h \<in> T \<and> h < t2})"
 
 (* define an observable memory on every location , every thread every time.
@@ -864,9 +1178,9 @@ inductive_set seqPos :: "time_type set \<Rightarrow> (time_type \<Rightarrow> ('
     and rho :: "(time_type \<Rightarrow> ('tid \<times> aid_type \<times> (aid_type, 'val, loc_type,
                  'lock, 'name, 'callID) action) option)"
     and Locs :: "loc_type set" where
-moSeqAtomic : "\<lbrakk> t \<in> T; rho t = Some (tid,aid,ac); isSeqAtomic ac; acLoc ac = Some x; x \<in> Locs\<rbrakk>
+moSeqAtomic : "\<lbrakk> t \<in> T;  isSeqAtomic rho t; getLoc rho t = Some x; x \<in> Locs;getTid rho t = Some tid\<rbrakk>
                 \<Longrightarrow> (tid,t,x) \<in> seqPos T rho Locs"
-| moSeqFence : "\<lbrakk> t \<in> T; rho t = Some (tid,aid,Fence SeqCst); x \<in> Locs\<rbrakk>
+| moSeqFence : "\<lbrakk> t \<in> T; isSeqFence rho t; x \<in> Locs; getTid rho t = Some tid\<rbrakk>
                 \<Longrightarrow> (tid,t,x) \<in> seqPos T rho Locs"
 
 definition hasPrevMem where
@@ -875,18 +1189,18 @@ definition hasPrevMem where
 definition hasReadFrom where
 "hasReadFrom T t rf = (\<exists> t' \<in> T . (t',t) \<in> rf)"
 
-definition samLocInMid where
-"samLocInMid T rho a b tid x =
-   (\<exists> t aid ac . a < t \<and> t < b \<and>  t \<in> T \<and> rho t = Some (tid,aid,ac) \<and> acLoc ac = Some x)"
+definition sameLocInMid where
+"sameLocInMid T rho a b tid x =
+   (\<exists> t . a < t \<and> t < b \<and>  t \<in> T \<and> getLoc rho t = Some x \<and> getTid rho t = Some tid)"
 
 definition seqPosInMid where
 "seqPosInMid T Tids rho Locs a b x =
             (\<exists> t tid . t \<in> T \<and> tid \<in> Tids \<and> a < t \<and> t < b \<and> (tid,t,x) \<in> seqPos T rho Locs)"
 
 fun sameMemContentAux where
-"sameMemContentAux (AWrite vol1 x y z axl1) (AWrite vol2 u v w axl2) = (if x = u \<and> y = v then True else False)"
-| "sameMemContentAux (RMW vol1 x y z axl1) (RMW vol2 u v w axl2) = (if x = u \<and> y = v then True else False)"
-| "sameMemContentAux (NWrite vol1 x y z n1 n2 axl1) (NWrite vol2 u v w n3 n4 axl2) = (if x = u \<and> y = v then True else False)"
+"sameMemContentAux (AWrite vol1 x y z) (AWrite vol2 u v w) = (if x = u \<and> y = v then True else False)"
+| "sameMemContentAux (RMW vol1 x y z) (RMW vol2 u v w) = (if x = u \<and> y = v then True else False)"
+| "sameMemContentAux (NWrite vol1 x y z n1 n2) (NWrite vol2 u v w n3 n4) = (if x = u \<and> y = v then True else False)"
 | "sameMemContentAux x y = False"
 
 definition sameMemContent :: "(time_type \<Rightarrow> ('tid \<times> aid_type \<times> (aid_type, 'val, loc_type,
@@ -898,104 +1212,183 @@ definition sameMemContent :: "(time_type \<Rightarrow> ('tid \<times> aid_type \
                 (\<forall> tid1 aid1 tid2 aid2 ac1 ac2 . rho1 a' = Some (tid1,aid1,ac1) \<and> rho2 b' = Some (tid2,aid2,ac2)
                             \<and> sameMemContentAux ac1 ac2)))"
 
+(* define observable memory, useful for proving mo order and
+    usage in proving properties about the whole executions for a program
 inductive_set observeMem :: "'tid set \<Rightarrow> time_type set
               \<Rightarrow> (time_type \<Rightarrow> ('tid \<times> aid_type \<times> (aid_type, 'val, loc_type,
                  'lock, 'name, 'callID) action) option)
                \<Rightarrow> ('tid \<Rightarrow> (time_type \<times> time_type) set option)
+               \<Rightarrow> ('tid \<Rightarrow> (time_type \<times> time_type) set option)
                \<Rightarrow> (time_type \<times> time_type) set
                \<Rightarrow> loc_type set \<Rightarrow>
-                           ('tid \<times> time_type \<times> loc_type \<times> time_type option) set"
+                           ('tid \<times> time_type \<times> loc_type \<times> time_type) set"
 for Tids :: "'tid set"
     and E :: "time_type set"
     and rho :: "(time_type \<Rightarrow> ('tid \<times> aid_type \<times> (aid_type, 'val, loc_type,
                  'lock, 'name, 'callID) action) option)"
     and sbs :: "('tid \<Rightarrow> (time_type \<times> time_type) set option)"
+    and dds :: "('tid \<Rightarrow> (time_type \<times> time_type) set option)"
     and rf :: "(time_type \<times> time_type) set"
      and Locs :: "loc_type set" where
- moBase1 : "\<lbrakk> tid \<in> Tids; t \<in> E; sbs tid = Some sb; \<not> hasPrevMem E t sb; rho t = Some (tid,aid,ac);
-                    isFenceLike ac; x \<in> Locs\<rbrakk> 
-                  \<Longrightarrow> (tid,t,x,None) \<in> observeMem Tids E rho sbs rf Locs"
-| moReadBase1 : "\<lbrakk> tid \<in> Tids; t \<in> E; sbs tid = Some sb; \<not> hasPrevMem E t sb;
-                  rho t = Some (tid,aid,ac); isPureRead ac; acLoc ac = Some x; \<not> hasReadFrom E t rf \<rbrakk> 
-                  \<Longrightarrow> (tid,t,x,None) \<in> observeMem Tids E rho sbs rf Locs"
+ moBase1 : "\<lbrakk> tid \<in> Tids; t \<in> E; sbs tid = Some sb; \<not> hasPrevMem E t sb; getTid rho t = Some tid;
+                    isFenceLike rho t; x \<in> Locs\<rbrakk> 
+                  \<Longrightarrow> (tid,t,x,0) \<in> observeMem Tids E rho sbs dds rf Locs"
+| moReadBase1 : "\<lbrakk> tid \<in> Tids; t \<in> E; sbs tid = Some sb; \<not> hasPrevMem E t sb; getTid rho t = Some tid;
+                      isPureRead rho t; getLoc rho t = Some x; \<not> hasReadFrom E t rf \<rbrakk> 
+                  \<Longrightarrow> (tid,t,x,0) \<in> observeMem Tids E rho sbs dds rf Locs"
 | moReadBase2 : "\<lbrakk> tid \<in> Tids; t \<in> E; sbs tid = Some sb; \<not> hasPrevMem E t sb; y \<in> Locs;
-                  rho t = Some (tid,aid,ac); \<not> isFenceLike ac; acLoc ac = Some x; x \<noteq> y \<rbrakk> 
-                  \<Longrightarrow> (tid,t,y,None) \<in> observeMem Tids E rho sbs rf Locs"
-| moWriteOther1 : "\<lbrakk> tid \<in> Tids; t \<in> E; rho t = Some (tid,aid,ac); y \<in> Locs;
-                    isAtomicWrite ac; acLoc ac = Some x; x \<noteq> y;
-                   (tid, t'', y, a) \<in> observeMem Tids E rho sbs rf Locs; t'' < t;
-                     \<not> samLocInMid E rho t'' t tid y;\<not> seqPosInMid E Tids rho Locs t'' t y\<rbrakk> 
+                  getTid rho t = Some tid; isMemOp rho t; getLoc rho t = Some x; x \<noteq> y \<rbrakk> 
+                  \<Longrightarrow> (tid,t,y,0) \<in> observeMem Tids E rho sbs dds rf Locs"
+| moWriteOther1 : "\<lbrakk> tid \<in> Tids; t \<in> E; y \<in> Locs; getTid rho t = Some tid;
+                    isWrite rho t; isAtomic rho t; getLoc rho t = Some x; x \<noteq> y;
+                   (tid, t'', y, a) \<in> observeMem Tids E rho sbs dds rf Locs; t'' < t;
+                     \<not> sameLocInMid E rho t'' t tid y;\<not> seqPosInMid E Tids rho Locs t'' t y\<rbrakk> 
                   \<Longrightarrow> (tid,t,y,a) \<in> observeMem Tids E rho sbs rf Locs"
-| moWriteOther2 : "\<lbrakk> tid \<in> Tids; t \<in> E; rho t = Some (tid,aid,ac); y \<in> Locs;
-                    isAtomicWrite ac; acLoc ac = Some x; x \<noteq> y; (tid',t'',y) \<in> seqPos E rho Locs;
-                   (tid', t'', y, a) \<in> observeMem Tids E rho sbs rf Locs; t'' < t;
-                     \<not> samLocInMid E rho t'' t tid y;\<not> seqPosInMid E Tids rho Locs t'' t y\<rbrakk> 
-                  \<Longrightarrow> (tid,t,y,a) \<in> observeMem Tids E rho sbs rf Locs"
-| moAtomicWrite : "\<lbrakk> tid \<in> Tids; t \<in> E; rho t = Some (tid,aid,ac);
-                    isAtomicWrite ac; acLoc ac = Some x \<rbrakk> 
-                  \<Longrightarrow> (tid,t,x,Some t) \<in> observeMem Tids E rho sbs rf Locs"
+| moWriteOther2 : "\<lbrakk> tid \<in> Tids; t \<in> E; y \<in> Locs; getTid rho t = Some tid; isAtomic rho t;
+                     isWrite rho t; getLoc rho t = Some x; x \<noteq> y; (tid',t'',y) \<in> seqPos E rho Locs;
+                   (tid', t'', y, a) \<in> observeMem Tids E rho sbs dds rf Locs; t'' < t;
+                     \<not> sameLocInMid E rho t'' t tid y;\<not> seqPosInMid E Tids rho Locs t'' t y\<rbrakk> 
+                  \<Longrightarrow> (tid,t,y,a) \<in> observeMem Tids E rho sbs dds rf Locs"
+| moAtomicWrite : "\<lbrakk> tid \<in> Tids; t \<in> E; getTid rho t = Some tid;
+                    isAtomic rho t; isWrite rho t; getLoc rho t = Some x \<rbrakk> 
+                  \<Longrightarrow> (tid,t,x,t) \<in> observeMem Tids E rho sbs dds rf Locs"
 | moNWriteBase : "\<lbrakk> tid \<in> Tids; t \<in> E; rho t = Some (tid,aid,NWrite vol v x t' cur num axl); num \<noteq> cur;
-                 sbs tid = Some sb; \<not> hasPrevMem E t sb\<rbrakk> 
-                  \<Longrightarrow> (tid,t,x,None) \<in> observeMem Tids E rho sbs rf Locs"
+                     sbs tid = Some sb; \<not> hasPrevMem E t sb\<rbrakk> 
+                  \<Longrightarrow> (tid,t,x,0) \<in> observeMem Tids E rho sbs dds rf Locs"
 | moNWriteNoUpdate : "\<lbrakk> tid \<in> Tids; t \<in> E; rho t = Some (tid,aid,NWrite vol v x t' cur num axl); num \<noteq> cur;
-                         (tid, t'', x, a) \<in> observeMem Tids E rho sbs rf Locs; t'' < t;
-                         \<not> samLocInMid E rho t'' t tid x; \<not> seqPosInMid E Tids rho Locs t'' t x \<rbrakk> 
-                  \<Longrightarrow> (tid,t,x,a) \<in> observeMem Tids E rho sbs rf Locs"
+                         (tid, t'', x, a) \<in> observeMem Tids E rho sbs dds rf Locs; t'' < t;
+                         \<not> sameLocInMid E rho t'' t tid x; \<not> seqPosInMid E Tids rho Locs t'' t x \<rbrakk> 
+                  \<Longrightarrow> (tid,t,x,a) \<in> observeMem Tids E rho sbs dds rf Locs"
 | moNWriteNoUpdateSeq : "\<lbrakk> tid \<in> Tids; t \<in> E; rho t = Some (tid,aid,NWrite vol v x t' cur num axl); num \<noteq> cur;
-                         (tid', t'', x, a) \<in> observeMem Tids E rho sbs rf Locs; t'' < t;
+                         (tid', t'', x, a) \<in> observeMem Tids E rho sbs dds rf Locs; t'' < t;
                         (tid',t'',x) \<in> seqPos E rho Locs;
-                         \<not> samLocInMid E rho t'' t tid x;\<not> seqPosInMid E Tids rho Locs t'' t x \<rbrakk> 
-                  \<Longrightarrow> (tid,t,x,a) \<in> observeMem Tids E rho sbs rf Locs"
+                         \<not> sameLocInMid E rho t'' t tid x;\<not> seqPosInMid E Tids rho Locs t'' t x \<rbrakk> 
+                  \<Longrightarrow> (tid,t,x,a) \<in> observeMem Tids E rho sbs dds rf Locs"
 | moNWriteUpdate : "\<lbrakk> tid \<in> Tids; t \<in> E; rho t = Some (tid,aid,NWrite vol v x t' num num axl) \<rbrakk> 
-                  \<Longrightarrow> (tid,t,x,Some t) \<in> observeMem Tids E rho sbs rf Locs"
-| moFenceLike1 : "\<lbrakk> tid \<in> Tids; t \<in> E; rho t = Some (tid,aid,ac); 
-                    isFenceLike ac; x \<in> Locs; ac \<noteq> Fence SeqCst;
-                  (tid, t'', x, a) \<in> observeMem Tids E rho sbs rf Locs; t'' < t;
-                   \<not> samLocInMid E rho t'' t tid x;\<not> seqPosInMid E Tids rho Locs t'' t x\<rbrakk> 
-                  \<Longrightarrow> (tid,t,x,a) \<in> observeMem Tids E rho sbs rf Locs"
-| moFenceLike2 : "\<lbrakk> tid \<in> Tids; t \<in> E; rho t = Some (tid,aid,ac); 
-                    isFenceLike ac; x \<in> Locs; ac \<noteq> Fence SeqCst;
-                  (tid', t'', x, a) \<in> observeMem Tids E rho sbs rf Locs; t'' < t;
+                  \<Longrightarrow> (tid,t,x,t) \<in> observeMem Tids E rho sbs dds rf Locs"
+| moFenceLike1 : "\<lbrakk> tid \<in> Tids; t \<in> E; getTid rho t = Some tid;
+                    isFenceLike rho t; x \<in> Locs; \<not> isSeqFence rho t;
+                  (tid, t'', x, a) \<in> observeMem Tids E rho sbs dds rf Locs; t'' < t;
+                   \<not> sameLocInMid E rho t'' t tid x;\<not> seqPosInMid E Tids rho Locs t'' t x\<rbrakk> 
+                  \<Longrightarrow> (tid,t,x,a) \<in> observeMem Tids E rho sbs dds rf Locs"
+| moFenceLike2 : "\<lbrakk> tid \<in> Tids; t \<in> E; rho t = Some (tid,aid,ac); getTid rho t = Some tid;
+                    isFenceLike rho t; \<not> isSeqFence rho t;  x \<in> Locs;
+                  (tid', t'', x, a) \<in> observeMem Tids E rho sbs dds rf Locs; t'' < t;
                     (tid',t'',x) \<in> seqPos E rho Locs;
                    \<not> samLocInMid E rho t'' t tid x;\<not> seqPosInMid E Tids rho Locs t'' t x\<rbrakk> 
                   \<Longrightarrow> (tid,t,x,a) \<in> observeMem Tids E rho sbs rf Locs"
-| moSeqFence : "\<lbrakk> tid \<in> Tids; t \<in> E; rho t = Some (tid,aid,Fence SeqCst); x \<in> Locs;
+| moSeqFence : "\<lbrakk> tid \<in> Tids; t \<in> E; isSeqFence rho t; getTid rho t = Some tid; x \<in> Locs;
                   (t'', x, t) \<in> cw E rho rf\<rbrakk> 
-                  \<Longrightarrow> (tid,t,x,Some t'') \<in> observeMem Tids E rho sbs rf Locs"
+                  \<Longrightarrow> (tid,t,x, t'') \<in> observeMem Tids E rho sbs rf Locs"
+*)
 
-(* first posibility: two executions are equivalence
-    if their memories are the same for a set locs infinitely often.
- Tid T rho sb rf*)
-definition inifOften where
-"inifOften Tid T Locs rho1 sb1 rf1 rho2 sb2 rf2 =
-     (\<forall> t \<in> T . (\<exists> t' \<in> T . t' > t \<and>
-          (\<forall> tid x . tid \<in> Tid \<and> x \<in> Locs \<longrightarrow>
-            (\<exists> a b .
-               (tid,t',x,a) \<in> observeMem Tid T rho1 sb1 rf1 Locs
-              \<and> (tid,t',x,b) \<in> observeMem Tid T rho2 sb2 rf2 Locs
-              \<and> sameMemContent rho1 a rho2 b))))"
+(* One of the good things in ATRCM is that we don't need to define a modification order.
+   For any execution, there exists a modification order, and we just need to retrieve that.*)
+(* define the modification order for a location x*)
+definition mox where
+"mox T rho = {(a,x,b) . {a,b} \<subseteq> T \<and> a < b \<and> sameLoc rho a b
+                  \<and> isWrite rho a \<and> isWrite rho b \<and> getLoc rho a = Some x}"
 
-definition firstEquiv where
-"firstEquiv Tid T Locs rho1 sb1 rf1 rho2 sb2 rf2 =
-   (validExecution Tid T rho1 sb1 rf1 \<and> validExecution Tid T rho2 sb2 rf2
-      \<and> inifOften Tid T Locs rho1 sb1 rf1 rho2 sb2 rf2)"
+definition moUnion where
+"moUnion T rho Locs = trancl {(a,b) . (\<exists> x \<in> Locs . (a,x,b) \<in> mox T rho)}"
 
-(* second posibility: two executions are equivalence
-    if their memories are the same for a set locs eventually always.
- Tid T rho sb rf*)
-definition evalAlways where
-"evalAlways Tid T Locs rho1 sb1 rf1 rho2 sb2 rf2 =
-     (\<exists> t \<in> T . (\<forall> t' \<in> T . t' > t \<and>
-          (\<forall> tid x . tid \<in> Tid \<and> x \<in> Locs \<longrightarrow>
-            (\<exists> a b .
-               (tid,t',x,a) \<in> observeMem Tid T rho1 sb1 rf1 Locs
-              \<and> (tid,t',x,b) \<in> observeMem Tid T rho2 sb2 rf2 Locs
-              \<and> sameMemContent rho1 a rho2 b))))"
+(* define all the locations in an execution *)
+definition theLocs where
+"theLocs T rho = {x. (\<exists> t \<in> T . getLoc rho t = Some x)}"
 
-definition secondEquiv where
-"secondEquiv Tid T Locs rho1 sb1 rf1 rho2 sb2 rf2 =
-   (validExecution Tid T rho1 sb1 rf1 \<and> validExecution Tid T rho2 sb2 rf2
-      \<and> evalAlways Tid T Locs rho1 sb1 rf1 rho2 sb2 rf2)"
+(* prove that coherence are in modification order. *)
+lemma SatMo :
+  fixes Tid T \<rho> sb rf Locs x tid a b t1 t2
+  assumes A1 : "validExecution Tid T \<rho> sbs dds rf"
+  and A2 : "Locs = theLocs T \<rho>"
+  and A3 : "sameThread \<rho> a b"
+  and A4 : "(t1,x, a) \<in> fullRf T \<rho> rf"
+  and A5 : "(t2,x, b) \<in> fullRf T \<rho> rf"
+  and A6 :  "a > b"
+  and A7 :  "t1 \<noteq> t2"
+  and A8 : "t1 \<in> T"
+  and A9 : "t2 \<in> T"
+shows "(t2,x,t1) \<in> (mox T \<rho>)"
+using A8 and A9
+proof (simp add: mox_def)
+  from A1
+  have B1 : "wellformedTime T \<rho> rf"
+  and B2: "wellformedTid Tid \<rho>" 
+  and B3 : "wellformedSB Tid T sbs"
+  and B4 : "wellformedRF T \<rho> rf"
+  and B5 : "rhoAssumption T \<rho>" 
+  and B6 : "rfAllAssumption rf \<rho>"
+  and B7 : "allSbAllAssumptions Tid sbs \<rho>"
+  and B8 : "locksProp T \<rho>" 
+  and B9 : "sat Tid T \<rho> sbs dds rf"
+    by (simp add: validExecution_def)+
+    show "t2 < t1 \<and>
+    (case \<rho> t2 of None \<Rightarrow> False | Some (xa, y, z) \<Rightarrow> (case \<rho> t1 of None \<Rightarrow> False | Some (u, v, x) \<Rightarrow> sameLocBasic z x)) \<and>
+    (case \<rho> t2 of None \<Rightarrow> False | Some (xa, y, x) \<Rightarrow> isWriteBasic x) \<and>
+    (case \<rho> t1 of None \<Rightarrow> False | Some (xa, y, x) \<Rightarrow> isWriteBasic x) \<and>
+              (case \<rho> t2 of None \<Rightarrow> None | Some (xa, y, x) \<Rightarrow> acLoc x) = Some x"
+    proof (rule_tac conjI)
+      from B9 and  A4 and A5 and A6 and A3
+      have LessEq : "t2 \<le> t1"
+        by (simp add: sat_le)
+      from A7 and LessEq
+      show "t2 < t1" by simp
+    next
+      from A4 and A5 and A8 and A9 and B1 and B4 and B5
+      have CrossSameLoc : "sameLoc \<rho> t2 t1"
+        by (rule_tac T = T and \<rho> = \<rho> and rf = rf and s = t2
+                       and a = b and t = t1 and b = a and x = x in sameLocTwoInFullRf,clarsimp+)
+      from A4 and B1 and B4 and B5
+      have AInT : "a \<in> T"
+        by (simp add: fullRfReadInSet)
+      from A5 and B1 and B4 and B5
+      have BInT : "b \<in> T"
+        by (simp add: fullRfReadInSet)
+      from A4 and A8 and AInT and B1 and B4 and B5
+      have IsWriteT1 : "isWrite \<rho> t1"
+        by (rule_tac T = T and \<rho> = \<rho> and rf = rf
+                       and a = t1 and b = a and x = x in isWriteInFullRf,clarsimp+)
+      from A5 and A9 and BInT and B1 and B4 and B5
+      have IsWriteT2 : "isWrite \<rho> t2"
+        by (rule_tac T = T and \<rho> = \<rho> and rf = rf
+                       and a = t2 and b = b and x = x in isWriteInFullRf,clarsimp+)
+      from A5 and A9 and BInT and B1 and B4 and B5
+      have GetLocT2 : "getLoc \<rho> b = Some x"
+        by (rule_tac T = T and \<rho> = \<rho> and rf = rf
+                       and a = t2 and b = b and x = x in locXInFullRf,clarsimp+)
+      from A5 and A9 and BInT and B1 and B4 and B5
+      have sameLocT2 : "sameLoc \<rho> t2 b"
+        by (rule_tac T = T and \<rho> = \<rho> and rf = rf
+                       and a = t2 and b = b and x = x in sameLocInFullRf,clarsimp+)
+      from A4 and A5 and A8 and A9 and B1 and B4 and B5
+      have CrossSameLoc : "sameLoc \<rho> t2 t1"
+        by (rule_tac T = T and \<rho> = \<rho> and rf = rf and s = t2
+                       and a = b and t = t1 and b = a and x = x in sameLocTwoInFullRf,clarsimp+)
+      from A4 and A5 and A8 and A9 and B1 and B4 and B5 and CrossSameLoc
+              and IsWriteT1 and IsWriteT2 and GetLocT2 and sameLocT2
+      show "(case \<rho> t2 of None \<Rightarrow> False | Some (xa, y, z) \<Rightarrow>
+                (case \<rho> t1 of None \<Rightarrow> False | Some (u, v, x) \<Rightarrow> sameLocBasic z x)) \<and>
+    (case \<rho> t2 of None \<Rightarrow> False | Some (xa, y, x) \<Rightarrow> isWriteBasic x) \<and>
+    (case \<rho> t1 of None \<Rightarrow> False | Some (xa, y, x) \<Rightarrow> isWriteBasic x)
+                \<and> (case \<rho> t2 of None \<Rightarrow> None | Some (xa, y, x) \<Rightarrow> acLoc x) = Some x"
+        apply (case_tac "\<rho> t2")
+         apply (simp add: wellformedTime_def rhoAssumption_def, clarsimp+)
+        apply (case_tac "\<rho> t1")
+         apply (simp add: wellformedTime_def wellformedRF_def rhoAssumption_def)
+        apply (case_tac "\<rho> b")
+         apply (simp add: wellformedTime_def wellformedRF_def rhoAssumption_def)
+        apply clarsimp
+        apply (case_tac "acLoc ba")
+         apply (simp add: wellformedTime_def wellformedRF_def rhoAssumption_def)
+        apply clarsimp
+        apply (case_tac "acLoc baa")
+         apply (simp add: wellformedTime_def wellformedRF_def rhoAssumption_def)
+        apply clarsimp
+        apply (case_tac "af = x")
+        by clarsimp+
+    qed
+  qed
+
 
 end
 
